modification to the code according to last meeting in CNAM

language_formal/spark2014_semantics/propertyProof.v
@@ -53,10 +53,8 @@ Proof.
     inversion h3;
     inversion h2; subst.
   - (* Econst *)
-    inversion H7; subst.
     constructor.
-  - inversion H7; subst.
-    constructor.  
+  - constructor.  
   - (* Evar *)
     specialize (typed_value _ _ i v h1 ); intros hz1.
     specialize (hz1 H6).
@@ -64,21 +62,17 @@ Proof.
     rewrite H3 in H. inversion H; subst.
     apply value_type_consistent; assumption.
   - (* Ebinop *)
-    specialize (IHe1 _ _ h1 H12 H5).
-    specialize (IHe2 _ _ h1 H14 H6).
+    specialize (IHe1 _ _ h1 H14 H5).
+    specialize (IHe2 _ _ h1 H15 H6).
     destruct v1 as [v11 | v12]; inversion IHe1; subst;
     destruct v2 as [v21 | v22]; try rm_contradict.
     + destruct b; 
        repeat simpl_binop_hyp; 
-       simpl; try constructor.
-       destruct (Zeq_bool v21 0).
-       * inversion H0.
-       * constructor.       
+       inversion H17; subst; constructor.
     + destruct b; try simpl_binop_hyp;
-       constructor.
+       inversion H17; subst; constructor.
   - (* Eunop *)
-    rewrite <- H8.
-    destruct op; destruct v0; inversion H8.
+    destruct op; destruct v0; inversion H9; subst.
     constructor.
 Qed.
 
@@ -100,10 +94,8 @@ Proof.
     inversion h3;
     inversion h2; subst.
   - (* Econst *)
-    inversion H7; subst.
     constructor.
-  - inversion H7; subst.
-    constructor.  
+  - constructor.  
   - (* Evar *)
     specialize (typed_value _ _ i v h1 ); intros hz1.
     specialize (hz1 H6).
@@ -111,666 +103,29 @@ Proof.
     rewrite H3 in H. inversion H; subst.
     apply value_type_consistent; assumption.
   - (* Ebinop *)
-    specialize (IHe1 _ _ h1 H12 H5).
-    specialize (IHe2 _ _ h1 H13 H6).
+    specialize (IHe1 _ _ h1 H14 H5).
+    specialize (IHe2 _ _ h1 H15 H6).
     destruct v1 as [v11 | v12]; inversion IHe1; subst;
     destruct v2 as [v21 | v22]; try rm_contradict.
     + destruct b; 
-       repeat simpl_binop_hyp; 
-       simpl; try constructor.
-       destruct (Zeq_bool v21 0).
-       * inversion H0.
-       * constructor.       
+       repeat simpl_binop_hyp;
+       inversion H18; subst; constructor.
     + destruct b; try simpl_binop_hyp;
-       constructor.
+       inversion H18; subst; constructor.
+  - specialize (IHe1 _ _ h1 H14 H5).
+    specialize (IHe2 _ _ h1 H15 H6).
+    destruct v1 as [v11 | v12]; inversion IHe1; subst;
+    destruct v2 as [v21 | v22]; try rm_contradict.
+    + destruct b; 
+       repeat simpl_binop_hyp;
+       inversion H17; subst; constructor.
+    + destruct b; try simpl_binop_hyp;
+       inversion H17; subst; constructor.
   - (* Eunop *)
-    rewrite <- H8.
-    destruct op; destruct v0; inversion H8.
+    destruct op; destruct v0; inversion H9; subst.
     constructor.
 Qed.
 
-(**************************************************************************)
-(**************************************************************************)
-
-(** some help lemmas *)
-Lemma valid_update: forall tb s ast_id x e v,
-    type_check_stack tb s ->
-    well_typed_stmt tb (Sassign ast_id x e) ->
-    exists s', update s x (Value v) = Some s'.
-Proof.
-    intros tb s ast_id x e v h1 h2.
-    inversion h2; subst.
-    specialize (typed_value' _ _ _ Out t h1 H2); intros hz1.
-    rm_exists.
-    clear h1 h2 H0 H2 H4.
-    functional induction (reside x s).
-    + unfold update; rewrite e1.
-       exists ((y, Value v) :: s'); auto.
-    + specialize (IHb H).
-       rm_exists.
-       unfold update.
-       rewrite e1.
-       fold update.
-       rewrite H0. 
-       exists ((y, v0) :: x0); auto.
-    + inversion H.
-Qed.
-
-(** update to the well-typed stack should return well-typed stack  *)
-Lemma type_reserve: forall s x v s' tb m t ,
-    update s x (Value v) = Some s' ->    
-    type_check_stack tb s -> 
-    lookup x tb = Some (m, t)-> 
-    return_value_type (ValNormal v) t ->
-    type_check_stack tb s'.
-Proof.
-    intros s x v.
-    remember (Value v) as v'0.
-    functional induction (update s x v'0);
-    intros s'0 tb m t h1 h2 h3 h4.
-  - inversion h1; clear h1; subst.
-    destruct tb. 
-    + inversion h3.
-    + destruct p.
-       inversion h2; subst;
-       unfold lookup in h3; rewrite e0 in h3; fold lookup;
-       inversion h3; clear h3; subst;
-       destruct v;
-       [ rm_contradict | | | rm_contradict | rm_contradict | | | rm_contradict ];
-       constructor; assumption.
-  - inversion h1; subst.
-    destruct tb.
-    + inversion h3.
-    + assert (hz1: Value v = Value v); auto.
-       destruct p; 
-       inversion h2; subst;
-       constructor;
-       unfold lookup in h3; rewrite e0 in h3; fold lookup in h3;
-       specialize (IHo hz1 _ _ _ _ e1 H0 h3 h4);
-       assumption.
-  - inversion h1.
-  - inversion h1.
-Qed.
-
-(** the resulting stack should be well-typed after the modification to the initially well-typed stack by the assignment *)
-Lemma type_reserve_assign: forall tb s ast_id x e v s',
-    type_check_stack tb s -> 
-    well_typed_stmt tb (Sassign ast_id x e) -> 
-    eval_expr s e (ValNormal v) ->
-    update s x (Value v) = Some s' ->
-    type_check_stack tb s'. 
-Proof.
-    intros tb s ast_id x e v s' h1 h2 h3 h4.
-    inversion h2; subst.
-    specialize (eval_type_reserve _ _ _ _ _ h1 h3 H4); intros hz1.
-    specialize (type_reserve _ _ _ _ _ _ _ h4 h1 H2 hz1); intros hz2.
-    assumption.
-Qed.
-
-(** the resulting state for executing a statement can be either exception or a 
-     normal state according to the semantics rules 
-*)
-Lemma symbol_consistent_reserve_0: forall tb s c s',
-    type_check_stack tb s -> 
-    well_typed_stmt tb c ->
-    eval_stmt s c s' -> 
-    s' = SException \/ (exists s0, s' = SNormal s0 /\ type_check_stack tb s0).
-Proof.
-    intros tb s c s' h1 h2 h3.
-    induction h3;
-    try match goal with
-    | [ |- SException = SException \/ _ ] => left; reflexivity
-    end.
-  - (* Sassign *)
-    right.
-    exists s1.
-    split.
-    reflexivity.
-    specialize (type_reserve_assign _ _ _ _ _ _ _ h1 h2 H H0); intros hz1.
-    assumption.
-  - (* Sseq *)
-    inversion h2; subst.
-    specialize (IHh3_1 h1 H2).
-    destruct IHh3_1 as [hz1 | hz1]; inversion hz1.
-    destruct H. 
-    inversion H; subst.
-    specialize (IHh3_2 H0 H4).
-    assumption.
-  - (* Sifthen_true *)
-    inversion h2; subst.
-    apply IHh3; assumption.
-  - (* Sifthen_false *)
-    right. 
-    exists s;
-    split; auto.
-  - (* Swhile_true *)
-    apply IHh3_2; auto.
-    inversion h2; subst.
-    specialize (IHh3_1 h1 H5).
-    destruct IHh3_1 as [hz1 | hz1]; inversion hz1.
-    destruct hz1. destruct H0.
-    inversion H0; subst. 
-    assumption.
-  - (* Swhile_false *)
-    right.
-    exists s; 
-    split; auto.
-Qed.
-
-(** 
-    if the initial stack is well-typed, and when we execute a command, 
-    the resulting normal stack should also be well-typed
-*)
-Lemma symbol_consistent_reserve: forall tb s c s',
-    type_check_stack tb s -> 
-    well_typed_stmt tb c ->
-    eval_stmt s c (SNormal s') -> 
-    type_check_stack tb s'. 
-Proof.
-    intros tb s c s' h1 h2 h3.
-    remember (SNormal s') as s1.
-    specialize (symbol_consistent_reserve_0 _ _ _ _ h1 h2 h3); intros hz1.
-    subst.
-    destruct hz1 as [hz2 | hz2]; inversion hz2.
-    destruct H.
-    inversion H; subst.
-    assumption.
-Qed.
-
-
-(** for any stack s, a corresponding initialization state map can be computed from it *)
-Lemma imap_exists: forall s, 
-    exists istate, initializationMap s istate.
-Proof.
-    intros s.
-    induction s.
-    exists nil; constructor.
-    rm_exists.
-    destruct a.
-    destruct v.
-  - exists ((i, Init) :: x); constructor. 
-    intuition. inversion H0.
-    assumption.
-  - exists ((i, Uninit) :: x); constructor.
-    auto.
-    assumption.
-Qed.
-
-(****************************************************)
-(****************************************************)
-
-(** 
-    if expression e is well-defined (meaning that all variables used in e has been initialized) under the 
-    initialization state map istate1, and for all variables that are initialized in istate1 are also initialized in istate2, 
-    then of course, e is also well-typed under istate2
-*)
-Lemma initializationMap_expr: forall istate1 e istate2,
-     well_defined_expr istate1 e ->   
-     (forall x, fetch2 x istate1 = Some Init -> fetch2 x istate2 = Some Init) ->
-     well_defined_expr istate2 e.
-Proof.
-    intros istate1 e istate2 h1.
-    generalize istate2. 
-    clear istate2.
-    induction e;
-    intros istate2 h2.
-  - destruct c; constructor.
-  - inversion h1; subst.
-    specialize (h2 _ H1).
-    constructor. assumption.
-  - inversion h1; subst.
-    constructor.
-    + specialize (IHe1 H2 _ h2).
-       assumption.
-    + specialize (IHe2 H5 _ h2).
-       assumption.
-  - inversion h1; subst.
-    constructor.
-    specialize (IHe H1 _ h2).
-    assumption.
-Qed.
-
-(* this modified version is used to prove lemma: ''initializationMap_stmt'' *)
-(** 
-    if expression e is well-defined (meaning that all variables used in e has been initialized) under the 
-    initialization state map istate1, and for all variables that are initialized in istate1 are also initialized in istate2, 
-    and for variables that are uninitialized in state1 may be initialized or uninitialized in istate2,
-    then of course, e is also well-typed under istate2
-*)
-Lemma initializationMap_expr1: forall istate1 e istate2,
-     well_defined_expr istate1 e ->   
-     (forall x, (fetch2 x istate1 = Some Init -> fetch2 x istate2 = Some Init) /\
-                   (fetch2 x istate1 = Some Uninit -> exists m, fetch2 x istate2 = Some m)) ->
-     well_defined_expr istate2 e.
-Proof.
-    intros.
-    distr_qualifier.
-    specialize (initializationMap_expr _ _ _ H H0); intros hz1.
-    assumption.
-Qed.
-
-(** 
-    if istate1 is a subset of istate2, which means that all variables that are initialized in istate1 are also
-    initialized in istate2, and istate2 is a subset of istate3, then istate1 is subset of istate3 
-*)
-Lemma fetch2_transitive: forall istate1 istate2 istate3,
-    (forall x : idnum,
-      (fetch2 x istate1 = Some Init -> fetch2 x istate2 = Some Init) /\
-      (fetch2 x istate1 = Some Uninit ->
-       exists m : init_mode, fetch2 x istate2 = Some m)) ->       
-    (forall x : idnum,
-      (fetch2 x istate2 = Some Init -> fetch2 x istate3 = Some Init) /\
-      (fetch2 x istate2 = Some Uninit ->
-       exists m : init_mode, fetch2 x istate3 = Some m)) ->
-    (forall x : idnum,
-      (fetch2 x istate1 = Some Init -> fetch2 x istate3 = Some Init) /\
-      (fetch2 x istate1 = Some Uninit ->
-       exists m : init_mode, fetch2 x istate3 = Some m)).
-Proof.
-    intros istate1 istate2 istate3 h1 h2.
-    intros x.
-    repeat distr_qualifier.
-    split; intros hz1.
-  - apply H0.
-    apply H2; assumption.
-  - specialize (H3 _ hz1).
-    rm_exists.
-    destruct x0 as [x1 | x2].
-    + specialize (H0 _ H).
-       exists Init; assumption.
-    + specialize (H1 _ H).
-       assumption.
-Qed.
-
-(* 'c' is put before 'istate1', because when we do induction on 'c', keep 'istate1' universal *)
-(** 
-    if command c is well-defined under both the initialization states istate1 and istate2 and 
-    istate1 is a subset of istate2, then the resulting initialization state istate1' should be the subset 
-    of istate2'
-*)
-Lemma wd_fetch2_sync: forall c istate1 istate1' istate2 istate2',
-    well_defined_stmt istate1 c istate1' ->
-    well_defined_stmt istate2 c istate2' ->
-    (forall x, (fetch2 x istate1 = Some Init -> fetch2 x istate2 = Some Init) /\
-                  (fetch2 x istate1 = Some Uninit -> exists m', fetch2 x istate2 = Some m')) ->
-    (forall x, (fetch2 x istate1' = Some Init -> fetch2 x istate2' = Some Init) /\
-                  (fetch2 x istate1' = Some Uninit -> exists m', fetch2 x istate2' = Some m')).
-Proof.
-    induction c;
-    intros istate1 istate1' istate2 istate2' h1 h2 h3.
-  - distr_qualifier.
-    inversion h1; subst.
-    inversion h2; subst.
-    intros x.
-    split; intros hz1.
-    + specialize (update2_in1 _ _ _ _ _ _ H7 hz1); intros hz2.
-       inversion hz2 as [hz3 | hz4].
-       * inversion hz3; subst.
-         specialize (update2_fetch2_new _ _ _ _  H9). 
-         auto.
-       * rm_exists.
-         specialize (H0 _ H2).
-         specialize (update2_fetch2_old _ _ _ _ _ H9 H); intros hz3.
-         rewrite H0 in hz3.
-         assumption.
-    + specialize (update2_in1 _ _ _ _ _ _ H7 hz1); intros hz2.
-       inversion hz2 as [hz3 | hz4].
-       * inversion hz3.
-          inversion H2.
-       * rm_exists.
-         specialize (H1 _ H2).
-         specialize (update2_fetch2_old _ _ _ _ _ H9 H); intros hz3.
-         rewrite hz3.
-         assumption.
-  - distr_qualifier.
-    inversion h1; subst.
-    inversion h2; subst.
-    intros x.
-    split; intros hz1.
-    specialize (H0 _ hz1); assumption.
-    specialize (H1 _ hz1); assumption.
-  - distr_qualifier.
-    inversion h1; subst.
-    inversion h2; subst.
-    intros x.
-    split; intros hz1.
-    specialize (H0 _ hz1); assumption.
-    specialize (H1 _ hz1); assumption.
-  - inversion h1; subst.
-    inversion h2; subst.
-    intros x.
-    split; intros hz1;
-    specialize (IHc1 _ _ _ _ H4 H6 h3);
-    specialize (IHc2 _ _ _ _ H5 H7 IHc1);
-    repeat distr_qualifier.
-    + apply H2. assumption.
-    + apply H3. assumption.
-Qed.
-
-(** 
-    if command c is well-defined under the initialization state istate1, and istate1 is a subset of  
-    istate2, then c should also be well-defined under istate2
-*)
-Lemma initializationMap_stmt: forall istate1 c istate1' istate2,
-     well_defined_stmt istate1 c istate1' ->   
-     (forall x, (fetch2 x istate1 = Some Init -> fetch2 x istate2 = Some Init) /\
-                   (fetch2 x istate1 = Some Uninit -> exists m, fetch2 x istate2 = Some m)) ->
-     exists istate2', well_defined_stmt istate2 c istate2'.
-Proof.
-    intros istate1 c istate1' istate2 h1.
-    generalize istate2. clear istate2.
-    induction h1;
-    intros istate2 h2.
-  - specialize (initializationMap_expr1 _ _ _ H h2); intros hz1.
-    assert (hz2: exists istate, update2 istate2 x Init = Some istate).
-    + distr_qualifier.
-       specialize (update2_fetch2 _ _ _ _ H0); intros hz2.
-       rm_exists. 
-       destruct x0.
-       * specialize (H2 _ H1).
-         specialize (fetch2_update2 _ _ _ Init H2); intros hz3.
-         assumption.
-       * specialize (H3 _ H1).
-         inversion H3.
-         specialize (fetch2_update2 _ _ _ Init H4); intros hz4.
-         assumption.
-    + rm_exists.
-       exists x0.
-       constructor; assumption.
-  - specialize (IHh1_1 _ h2).
-    rm_exists.
-    assert (hz2: forall y : idnum, (fetch2 y s' = Some Init -> fetch2 y x = Some Init) /\ 
-                                                 (fetch2 y s' = Some Uninit -> exists m', fetch2 y x = Some m')).
-    + specialize (wd_fetch2_sync _ _ _ _ _ h1_1 H h2); intros hz1.
-       assumption.
-    + specialize (IHh1_2 x hz2).
-       rm_exists.
-       exists x0.
-       apply WD_Sseq with (s' := x);
-       assumption.
-  - exists istate2.
-    specialize (IHh1 _ h2).
-    rm_exists.
-    apply WD_Sifthen with (s' := x).    
-    + distr_qualifier.
-       specialize (initializationMap_expr _ _ _ H H2); intros hz1.
-       assumption.
-    + assumption.
-  - exists istate2.
-    specialize (IHh1 _ h2).
-    rm_exists.
-    apply WD_Swhile with (s' := x).
-    + distr_qualifier.
-       specialize (initializationMap_expr _ _ _ H H2); intros hz1.
-       assumption.
-    + assumption.
-Qed.
-
-(** 
-    command may change the uninitialized variables into initialized ones, 
-    so the initialization state istate before executing command c should be
-    subset of the resulting initialization state istate'
-*)
-Lemma initializationMap_inc: forall istate c istate',
-     well_defined_stmt istate c istate' ->   
-     (forall x, (fetch2 x istate = Some Init -> fetch2 x istate' = Some Init) /\
-                   (fetch2 x istate = Some Uninit -> exists m, fetch2 x istate' = Some m)).
-Proof.
-    intros istate c istate' h1.
-    induction h1; 
-    intros x0.
-  - split; intros;
-    remember (beq_nat x0 x) as eq;
-    symmetry in Heqeq;
-    destruct eq as [eq1 | eq2].
-       * apply beq_nat_true in Heqeq.
-         subst.
-         specialize (update2_fetch2_new _ _ _ _ H0); intros hz1.
-         assumption.
-       * apply beq_nat_false in Heqeq.
-         specialize (update2_fetch2_old _ _ _ _ _ H0 Heqeq); intros hz1.
-         rewrite hz1.
-         assumption.
-       * apply beq_nat_true in Heqeq.
-         subst.
-         specialize (update2_fetch2_new _ _ _ _ H0); intros hz1.
-         exists Init; assumption.
-       * apply beq_nat_false in Heqeq.
-         specialize (update2_fetch2_old _ _ _ _ _ H0 Heqeq); intros hz1.
-         rewrite hz1.
-         exists Uninit; assumption.         
-  - repeat distr_qualifier.
-    split; intros hz1.
-    + apply H0.
-       apply H2.
-       assumption.
-    + specialize (H3 _ hz1).
-       rm_exists.
-       destruct x.
-       specialize (H0 _ H).
-       exists Init; assumption.
-       specialize (H1 _ H).
-       assumption.
-  - split.
-    + auto.
-    + intros.
-       exists Uninit.
-       assumption.
-  - split.
-    + auto.
-    + intros.
-       exists Uninit.
-       assumption.
-Qed.
-
-Ltac rm_hyps := 
-    match goal with
-    | [ h: SNormal _ = SException \/ _ |- _] => destruct h as [h1z | h2z]; [inversion h1z | intuition] 
-    end.
-
-(** 
-    in well_defined_stmt, the initialization state istate' after executing the conditional and while statement is 
-    defined as the intersection of the resulting initialization states from both branches;
-    in eval_stmt, it executes either true branch or false branch for conditional and while statemet according
-    to the current state s,  so the initialization state istate1 computed from s' should be a superset of istate'
- *)
-Lemma eval_stmt_greater_0: forall s c s' istate istate' s0 istate1,
-     eval_stmt s c s' ->
-     initializationMap s istate ->
-     well_defined_stmt istate c istate' -> 
-     s' = SException \/ 
-     (s' = SNormal s0 /\ initializationMap s0 istate1 -> 
-     (forall x, (fetch2 x istate' = Some Init -> fetch2 x istate1 = Some Init) /\
-                   (fetch2 x istate' = Some Uninit -> exists m, fetch2 x istate1 = Some m))).
-Proof.
-    intros s c s' istate istate' s0 istate1 h1.
-    generalize istate istate' s0 istate1.
-    clear istate istate' s0 istate1.
-    induction h1;
-    intros istate istate' s0 istate1 h2 h3;
-    try match goal with
-    | [ |- SException = SException \/ _ ] => left; reflexivity
-    end.
-  - (* 1. Sassign *)
-    right; intros h4.
-    inversion h3; subst.
-    destruct h4.
-    inversion H1; subst.
-    specialize (update_consis _ _ _ _ _ _ _ h2 H0 H7 H2); intros hz1.
-    subst.
-    intros. 
-    split; intros.
-    + assumption.
-    + exists Uninit.
-       assumption.
-  - (* 2. Sseq *)
-    inversion h3; subst.
-    specialize (imap_exists s1); intros hz1.
-    rm_exists.
-    specialize (IHh1_1 _ _ s1 x h2 H4).
-    rm_hyps.
-    assert (hz2: exists istate, well_defined_stmt x c2 istate).
-    specialize (initializationMap_stmt _ _ _ _ H5 H0); intros hz2.
-    assumption.
-    rm_exists.
-    specialize (IHh1_2 _ _ s0 istate1 H H1).
-    intuition. right.
-    intros H2. destruct H2.
-    specialize (H3 H2 H6).
-    specialize (wd_fetch2_sync _ _ _ _ _ H5 H1 H0); intros hz3.
-    specialize (fetch2_transitive _ _ _ hz3 H3); intros hz4.
-    assumption.
-  - (* 3. Sifthen_true *)
-    inversion h3; subst.
-    specialize (IHh1 _ _ s0 istate1 h2 H6).
-    specialize (initializationMap_inc _ _ _ H6); intros hz1.
-    destruct IHh1. left; assumption.
-    right; intros H2.
-    specialize (H0 H2).
-    specialize (fetch2_transitive _ _ _ hz1 H0); intros hz2.
-    assumption.
-  - (* 4. Sifthen_false *)
-    inversion h3; subst.
-    right; intros H2.
-    destruct H2. inversion H0; subst.
-    specialize (initializationMap_unique _ _ _ H1 h2); intros hz3.
-    subst. 
-    intuition. 
-    exists Uninit; auto.
-  - (* 5. Swhile_true *)
-    inversion h3; subst.
-    specialize (imap_exists s1); intros hz1.
-    rm_exists.
-    specialize (IHh1_1 _ _ s1 x h2 H6).
-    specialize (initializationMap_inc _ _ _ H6); intros hz2.
-    assert (hz2': exists istate, well_defined_stmt x (Swhile ast_id b c) istate).
-    exists x.
-    assert (hz3: exists istate, well_defined_stmt x c istate).
-    specialize (initializationMap_stmt _ _ _ _ H6 hz2); intros hz3.
-    inversion hz3.
-    rm_hyps.
-    specialize (initializationMap_stmt _ _ _ _ H1 H2); intros hz4.    
-    assumption.
-    inversion hz3.
-    apply WD_Swhile with (s' := x0). 
-    + rm_hyps.
-       specialize (fetch2_transitive _ _ _ hz2 H2); intros hz5.
-       specialize (initializationMap_expr1 _ _ _ H5 hz5); intros hz6.
-       assumption.
-    + assumption.
-    + inversion hz2'.
-       inversion H1; subst.
-       specialize (IHh1_2 _ _ s0 istate1 H0 H1).
-       destruct IHh1_2. left; assumption.
-       right; intros H3. 
-       specialize (H2 H3).
-       destruct IHh1_1. inversion H4.
-       assert (hz5: SNormal s1 = SNormal s1 /\ initializationMap s1 x0).
-       split; auto.
-       specialize (H4 hz5).
-       specialize (fetch2_transitive _ _ _ H4 H2); intros hz3.
-       specialize (fetch2_transitive _ _ _ hz2 hz3); intros hz4.
-       assumption.
-  - (* 6. Swhile_false *)
-    inversion h3; subst.
-    right; intros.
-    destruct H0. inversion H0; subst.
-    specialize (initializationMap_unique _ _ _ H1 h2); intros hz3.
-    subst.
-    split; intuition.
-    exists Uninit; auto.
-Qed.
-
-(** 
-    it's similar to eval_stmt_greater_0, the only difference is that we exclude the
-    exception state when running eval_stmt here 
-*)
-Lemma eval_stmt_greater: forall s c s' istate istate' istate1,
-     eval_stmt s c (SNormal s') -> 
-     initializationMap s istate ->
-     well_defined_stmt istate c istate' -> 
-     initializationMap s' istate1 -> 
-     (forall x, (fetch2 x istate' = Some Init -> fetch2 x istate1 = Some Init) /\
-                   (fetch2 x istate' = Some Uninit -> exists m, fetch2 x istate1 = Some m)).
-Proof.
-    intros s c s' istate istate' istate1 h1 h2 h3 h4.
-    remember (SNormal s') as s1.
-    specialize (eval_stmt_greater_0 _ _ _ _ _ s' istate1 h1 h2 h3); intros hz1.
-    destruct hz1.
-  - subst. inversion H.
-  - apply H; auto.
-Qed.
-
-(** 
-    according to the lemma eval_stmt_greater, we know that istate' is a subset of istate1, 
-    so whenever c2 is well-defined under istate', it should also be well-defined under istate1
-*)
-Lemma initializationMap_consistent: forall s istate c1 s' istate' c2 istate'' istate1,
-     initializationMap s istate ->
-     eval_stmt s c1 (SNormal s') -> 
-     well_defined_stmt istate c1 istate' -> 
-     well_defined_stmt istate' c2 istate'' ->      
-     initializationMap s' istate1 ->
-     exists istate2, well_defined_stmt istate1 c2 istate2.
-Proof.
-    intros s istate c1 s' istate' c2 istate'' istate1 h1 h2 h3 h4 h5.
-    specialize (eval_stmt_greater _ _ _ _ _ _ h2 h1 h3 h5); intros hz1.
-    specialize (initializationMap_stmt _ _ _ _ h4 hz1); intros hz2.
-    assumption.
-Qed.
-
-
-(* - - - - - - - - - - - - - - - - - - - - - - - - - - - - - - - - - - - - - - - - - - - - - - - - - - - -*)
-(* - - - - - - - - - - - - - - - - - - - - - - - - - - - - - - - - - - - - - - - - - - - - - - - - - - - -*)
-
-(** * Correctness Proof About Well-Formed Command *)
-
-(** 
-    subset is introduced to prove eval_expr_with_checks_correct and eval_stmt_with_checks_correct, 
-    otherwise they cannot be proved directly 
-*)
-Definition subset (cks1: check_points) (cks2: check_points): Prop := 
-    forall id ck, fetch_ck id cks1 = Some ck -> fetch_ck id cks2 = Some ck.
-
-Lemma subset_refl: forall ls,
-    subset ls ls.
-Proof.
-    intros.
-    unfold subset; intros.
-    assumption.
-Qed.
-
-Lemma subset_trans: forall cks0 cks1 cks2,
-    subset cks0 cks1 ->
-    subset cks1 cks2 ->
-    subset cks0 cks2.
-Proof.
-    intros.
-    unfold subset in *.
-    intros.
-    apply H0. apply H.
-    assumption.
-Qed.
-
-(** 
-    if all ast id numbers in checks list ls is less then n, in other words, n is outside the  
-   domain of ls, then when we fetch n from ls, of course it returns None
-*)
-Lemma fetch_ck_none: forall ls n,
-    ast_ids_lt ls n ->
-    fetch_ck n ls = None.
-Proof.
-    intros.
-    induction H.
-    + simpl. 
-       remember (beq_nat n ast_id) as b.
-       destruct b.
-       * symmetry in Heqb. 
-         apply beq_nat_true in Heqb; rewrite Heqb in H0.
-         omega.
-      * assumption.
-    + auto.
-Qed.
 
 Lemma lt_not_equal: forall x y,
     x < y ->
@@ -796,245 +151,113 @@ Proof.
     apply IHx.
 Qed.
 
-(** 
-   ast_id_inc_expr enforces that all ast id numbers used in expression e are unique and they are increasing,
-   cks1 stores the checks (indexed by ast id numbers) that are generated for expression e on top of cks0, 
-   if fetch n from cks0 is None and n is smaller than all ast id numbers in expression e, then fetch n 
-   from cks1 should also be None
-*)
-Lemma check_update_expr: forall cks0 e cks1 max n, 
-    check_generator_expr cks0 e cks1 ->
-    ast_id_inc_expr e max ->
-    fetch_ck n cks0 = None ->
-    n < get_ast_id_expr e ->
-    fetch_ck n cks1 = None.
-Proof.
-    intros cks0 e cks1 max n h1.
-    revert max n.
-    induction h1;
-    intros max n0 h2 h3 h4;
-    simpl in *;
-    specialize (lt_not_equal _ _ h4); intros hz1;
-    rewrite hz1;
-    auto.
-  - inversion h2; subst.
-    assert (hz2: n0 < get_ast_id_expr e1); intuition.
-    assert (hz3: n0 < get_ast_id_expr e2); intuition.
-    specialize (IHh1_1 _ _ H4 h3 hz2).
-    specialize (IHh1_2 _ _ H5 IHh1_1 hz3);
-    assumption.
-  - inversion h2; subst.
-    assert (hz2: n0 < get_ast_id_expr e); intuition.
-    specialize (IHh1 _ _ H2 h3 hz2).
-    assumption.
-Qed.
-
-(** it's similar to check_update_expr *)
-Lemma check_update_stmt: forall cks0 c cks1 max n, 
-    check_generator_stmt cks0 c cks1 ->
-    ast_id_inc_stmt c max ->
-    fetch_ck n cks0 = None ->
-    n < get_ast_id_stmt c ->
-    fetch_ck n cks1 = None.
-Proof.
-    intros cks0 c cks1 max n h1.
-    revert max n.
-    induction h1;
-    intros max n0 h2 h3 h4;
-    simpl in *;
-    specialize (lt_not_equal _ _ h4); intros hz1;
-    rewrite hz1;
-    inversion h2; subst;
-    auto.
-  - assert (hz: n0 < get_ast_id_expr e); intuition.
-    specialize (check_update_expr _ _ _ _ _ H H3 h3 hz); intros hz2.
-    assumption.
-  - assert (hz_1: n0 < get_ast_id_stmt c1); intuition.
-    assert (hz_2: n0 < get_ast_id_stmt c2); intuition.
-    specialize (IHh1_1 _ _ H2 h3 hz_1).
-    specialize (IHh1_2 _ _ H3 IHh1_1 hz_2).
-    assumption.
-  - assert (hz_1: n0 < get_ast_id_expr b); intuition.
-    assert (hz_2: n0 < get_ast_id_stmt c); intuition.
-    specialize (check_update_expr _ _ _ _ _ H H3 h3 hz_1); intros hz2.
-    specialize (IHh1 _ _ H4 hz2 hz_2); assumption.
-  - assert (hz_1: n0 < get_ast_id_expr b); intuition.
-    assert (hz_2: n0 < get_ast_id_stmt c); intuition.
-    specialize (check_update_expr _ _ _ _ _ H H3 h3 hz_1); intros hz2.
-    specialize (IHh1 _ _ H4 hz2 hz_2); assumption.
-Qed.
+(** * Correctness Proof About Well-Formed Command *)
 
 (** 
-    if ls0 is a subset of ls1 and x has never appeared in ls1, 
-    then, ls0 should be a subset of the ls1 added with new element indexed by x 
+    subset is introduced to prove eval_expr_with_checks_correct and eval_stmt_with_checks_correct, 
+    otherwise they cannot be proved directly 
 *)
-Lemma check_update: forall x ls1 ls0 flag,
-    fetch_ck x ls1 = None ->
-    subset ls0 ls1 ->
-    subset ls0 ((x, flag) :: ls1).
+Definition subset (n: astnum) (cks1: check_points) (cks2: check_points): Prop := 
+    forall id v, 
+    id < n -> 
+    fetch_ck id cks1 = v -> 
+    fetch_ck id cks2 = v.
+
+Lemma subset_refl: forall n ls,
+    subset n ls ls.
 Proof.
     intros.
-    unfold subset in *; intros.
-    unfold fetch_ck.
-    remember (beq_nat id x) as b.
-    destruct b.
-  - specialize (H0 _ _ H1).
-    symmetry in Heqb.
-    apply beq_nat_true in Heqb; subst.
-    rewrite H in H0; inversion H0.
-  - fold fetch_ck.
-    apply H0.
+    unfold subset; intros.
     assumption.
 Qed.
 
-Lemma sub_subset: forall x ls0 flag ls1,
-    fetch_ck x ls0 = None ->
-    subset ((x, flag) :: ls0) ls1 ->
-    subset ls0 ls1.
+
+Lemma subset_close: forall n0 n ls1 ls2,
+    subset n0 ls1 ls2 ->
+    n < n0 ->
+    subset n ls1 ls2.
 Proof.
     intros.
-    unfold subset in *;
+    unfold subset in *.
     intros.
-    apply H0.
-    simpl.
-    remember (beq_nat id x) as b.
-    destruct b.
-  - symmetry in Heqb.
-    apply beq_nat_true in Heqb; subst.
-    rewrite H in H1; inversion H1.
-  - assumption.    
+    apply H;
+    intuition.
 Qed. 
 
-
-(** 
-    cks1 is a list of checks that are generated for expression e on top of cks0, so cks1 
-    should be a superset of cks0;
-    ast_id_inc_expr enforces that all ast id numbers used in e are unique and increasing,
-    and ast_id_lt constrains that all ast ids in cks0 is smaller than the ast ids used in e, 
-    this is an implicit requirement enforced by check_generator_expr, for example: 
-    for binary expression e1 op e2, [check_generator_expr nil (e1 op e2) cks1] can be computed
-    by [check_generator_expr nil e1 cks0]  and [check_generator_expr cks0 e2 cks1], because the 
-    ast ids are increasing inside the expression, so all ast ids in cks0 should be smaller than the ast ids in e2;
-*)
-Lemma subset_expr: forall cks0 e cks1 max,
-    check_generator_expr cks0 e cks1 ->
-    ast_ids_lt cks0 (get_ast_id_expr e) -> (* make sure that all ast num used in e is fresh *)
-    ast_id_inc_expr e max -> (* make sure that all ast numbers are unique and increase *)
-    subset cks0 cks1.
+Lemma subset_close_le: forall n0 n ls1 ls2,
+    subset n0 ls1 ls2 ->
+    n <= n0 ->
+    subset n ls1 ls2.
 Proof.
-    intros cks0 e cks1 max h1 h2.
-    revert max.
-    induction h1; simpl in h2;
-    intros max h3.
-  - inversion h3; subst.
-    unfold subset; intros.
-    simpl. 
-    remember (beq_nat id max) as b.
-    destruct b.
-    symmetry in Heqb; apply beq_nat_true in Heqb; subst.
-    specialize (fetch_ck_none _ _ h2); intros hz1.
-    rewrite hz1 in H0; inversion H0.
-    auto.
-  - inversion h3; subst.
-    unfold subset; intros.
-    simpl. 
-    remember (beq_nat id max) as b.
-    destruct b.
-    symmetry in Heqb; apply beq_nat_true in Heqb; subst.
-    specialize (fetch_ck_none _ _ h2); intros hz1.
-    rewrite hz1 in H0; inversion H0.
-    auto.
-  - inversion h3; subst.
-    specialize (ast_ids_lt_trans _ _ _ h2 H9); intros hz1.
-    specialize (ast_ids_lt_trans _ _ _ h2 H10); intros hz2.
-    specialize (IHh1_1 hz1 _ H4).
-    specialize (ast_id_max_expr _ _ _ _ H4 h1_1 hz1); intros hz3.
-    assert (hz: max1 + 1 <= get_ast_id_expr e2); intuition.
-    specialize (ast_ids_lt_trans0 _ _ _ hz3 hz); intros hz4.
-    specialize (IHh1_2 hz4 _ H5).
-    specialize (subset_trans _ _ _ IHh1_1 IHh1_2); intros hz5.
+    intros.
+    unfold subset in *.
+    intros.
+    apply H;
+    intuition.
+Qed. 
 
-    specialize (fetch_ck_none _ _ h2); intros h1_3.
-    specialize (check_update_expr _ _ _ _ _ h1_1 H4 h1_3 H9); intros h1_4.
-    specialize (check_update_expr _ _ _ _ _ h1_2 H5 h1_4 H10); intros h1_5.
-    specialize (check_update _ _ _ flag h1_5 hz5); intros hz6.
-    assumption. 
-  - inversion h3; subst.
-    specialize (ast_ids_lt_trans _ _ _ h2 H5); intros hz1.
-    specialize (IHh1 hz1 _ H2).
-    unfold subset; intros.
-    simpl. 
-    remember (beq_nat id ast_id) as b.
-    destruct b.
-    symmetry in Heqb; apply beq_nat_true in Heqb; subst.
-    specialize (fetch_ck_none _ _ h2); intros hz2.
-    rewrite hz2 in H0; inversion H0.
-    apply IHh1. assumption.
+Lemma subset_close1: forall ls0 ls1 ast_id flag,
+    subset ast_id ((ast_id, flag) :: ls0) ls1 ->
+    subset ast_id ls0 ls1.
+Proof.
+    intros.
+    unfold subset in *.
+    intros.
+    apply H.
+    assumption.
+    specialize (lt_not_equal _ _ H0); intros hz1.
+    unfold fetch_ck.
+    rewrite hz1; fold fetch_ck.
+    assumption.
 Qed.
 
 
-(** it's similar to subset_expr *)
-Lemma subset_stmt: forall cks0 c cks1 max,
-    check_generator_stmt cks0 c cks1 ->
-    ast_ids_lt cks0 (get_ast_id_stmt c) -> 
-    ast_id_inc_stmt c max ->
-    subset cks0 cks1.
+Lemma subset_trans: forall n0 n1 cks0 cks1 cks2,
+    subset n0 cks0 cks1 ->
+    subset n1 cks1 cks2 ->
+    n0 < n1 ->
+    subset n0 cks0 cks2.
 Proof.
-    intros cks0 c cks1 max h1.
-    revert max.
-    induction h1; 
-    intros max h2 h3;
-    simpl in h2; inversion h3; subst.
-  - (* Sassign *)
-    specialize (ast_ids_lt_trans _ _ _ h2 H6); intros hz1.
-    specialize (subset_expr _ _ _ _ H hz1 H3); intros hz2.
-    
-    specialize (fetch_ck_none _ _ h2); intros h1_1.
-    specialize (check_update_expr _ _ _ _ _ H H3 h1_1 H6); intros h1_2.
-    specialize (check_update _ _ _ No_Check h1_2 hz2); intros hz3.
-    assumption.
-  - (* Sseq *)
-    specialize (ast_ids_lt_trans _ _ _ h2 H6); intros hz1.
-    specialize (IHh1_1 _ hz1 H2).
-    specialize (ast_id_max_stmt _ _ _ _ H2 h1_1 hz1); intros hz2.
-    assert (hz: max1 + 1 <= get_ast_id_stmt c2); intuition.
-    specialize (ast_ids_lt_trans0 _ _ _ hz2 hz); intros hz3.
-    specialize (IHh1_2 _ hz3 H3).
-    specialize (subset_trans _ _ _ IHh1_1 IHh1_2); intros hz4.
-    
-    specialize (fetch_ck_none _ _ h2); intros h1_3.
-    specialize (check_update_stmt _ _ _ _ _ h1_1 H2 h1_3 H6); intros h1_4.
-    specialize (check_update_stmt _ _ _ _ _ h1_2 H3 h1_4 H8); intros h1_5.
-    specialize (check_update _ _ _ No_Check h1_5 hz4); intros hz5.
-    assumption.
-  - (* Sifthen *)
-    specialize (ast_ids_lt_trans _ _ _ h2 H7); intros hz1.
-    specialize (ast_id_max_expr _ _ _ _ H3 H hz1); intros hz2.
-    assert (hz: max1 + 1 <= get_ast_id_stmt c); intuition.
-    specialize (ast_ids_lt_trans0 _ _ _ hz2 hz); intros hz3.
-    specialize (IHh1 _ hz3 H4).
-    specialize (subset_expr _ _ _ _ H hz1 H3); intros hz4.
-    specialize (subset_trans _ _ _ hz4 IHh1); intros hz5.
-    
-    specialize (fetch_ck_none _ _ h2); intros h1_3.
-    specialize (check_update_expr _ _ _ _ _ H H3 h1_3 H7); intros h1_4.
-    specialize (check_update_stmt _ _ _ _ _ h1 H4 h1_4 H9); intros h1_5.
-    specialize (check_update _ _ _ No_Check h1_5 hz5); intros hz6.
-    assumption.    
-  - (* Swhile *)
-    specialize (ast_ids_lt_trans _ _ _ h2 H7); intros hz1.
-    specialize (ast_id_max_expr _ _ _ _ H3 H hz1); intros hz2.
-    assert (hz: max1 + 1 <= get_ast_id_stmt c); intuition.
-    specialize (ast_ids_lt_trans0 _ _ _ hz2 hz); intros hz3.
-    specialize (IHh1 _ hz3 H4).
-    specialize (subset_expr _ _ _ _ H hz1 H3); intros hz4.
-    specialize (subset_trans _ _ _ hz4 IHh1); intros hz5.
+    intros.
+    unfold subset in *.
+    intros.
+    apply H0. 
+    intuition.
+    apply H; assumption.
+Qed.
 
-    specialize (fetch_ck_none _ _ h2); intros h1_3.
-    specialize (check_update_expr _ _ _ _ _ H H3 h1_3 H7); intros h1_4.
-    specialize (check_update_stmt _ _ _ _ _ h1 H4 h1_4 H9); intros h1_5.
-    specialize (check_update _ _ _ No_Check h1_5 hz5); intros hz6.
-    assumption.     
+Lemma subset_trans_le: forall n0 n1 cks0 cks1 cks2,
+    subset n0 cks0 cks1 ->
+    subset n1 cks1 cks2 ->
+    n0 <= n1 ->
+    subset n0 cks0 cks2.
+Proof.
+    intros.
+    unfold subset in *.
+    intros.
+    apply H0. 
+    intuition.
+    apply H; assumption.
+Qed.
+
+(** 
+    if all ast id numbers in checks list ls is less then n, in other words, n is outside the  
+   domain of ls, then when we fetch n from ls, of course it returns None
+*)
+Lemma fetch_ck_none: forall ls n,
+    ast_ids_lt ls n ->
+    fetch_ck n ls = None.
+Proof.
+    intros.
+    induction H.
+    + simpl. 
+       remember (beq_nat n ast_id) as b.
+       destruct b.
+       * symmetry in Heqb. 
+         apply beq_nat_true in Heqb; rewrite Heqb in H0.
+         omega.
+      * assumption.
+    + auto.
 Qed.
 
 (** 
@@ -1073,44 +296,143 @@ Qed.
 
 
 (** 
-    help1 and help2 are just help lemmas that are used repeatedly to prove eval_expr_with_checks_correct0, 
-    so I define them as lemmas
+    cks1 is a list of checks that are generated for expression e on top of cks0, so cks1 
+    should be a superset of cks0;
+    ast_id_inc_expr enforces that all ast id numbers used in e are unique and increasing,
+    and ast_id_lt constrains that all ast ids in cks0 is smaller than the ast ids used in e, 
+    this is an implicit requirement enforced by check_generator_expr, for example: 
+    for binary expression e1 op e2, [check_generator_expr nil (e1 op e2) cks1] can be computed
+    by [check_generator_expr nil e1 cks0]  and [check_generator_expr cks0 e2 cks1], because the 
+    ast ids are increasing inside the expression, so all ast ids in cks0 should be smaller than the ast ids in e2;
 *)
-Lemma help1: forall ls0 ls1 ls2 ast_id e1 e2 max1 max2,
-    ast_ids_lt ls0 ast_id ->
-    ast_id < get_ast_id_expr e1 -> 
-    max1 < get_ast_id_expr e2 -> 
-    check_generator_expr ls0 e1 ls1 ->
-    check_generator_expr ls1 e2 ls2 -> 
-    ast_id_inc_expr e1 max1 ->
-    ast_id_inc_expr e2 max2 -> 
-    subset ls1 ls2.
+Lemma subset_expr: forall cks0 e cks1 max,
+    check_generator_expr cks0 e cks1 ->
+    ast_ids_lt cks0 (get_ast_id_expr e) -> (* make sure that all ast num used in e is fresh *)
+    ast_id_inc_expr e max -> (* make sure that all ast numbers are unique and increase *)
+    subset (get_ast_id_expr e) cks0 cks1.
 Proof.
-    intros.
-    specialize (ast_ids_lt_trans _ _ _ H H0); intros hz1.
-    specialize (lt_trans_expr _ _ _ _ _ H2 hz1 H4 H1); intros hz2.
-    specialize (subset_expr _ _ _ _ H3 hz2 H5); intros hz5.
-    assumption.
+    intros cks0 e cks1 max h1 h2.
+    revert max.
+    induction h1; simpl in h2;
+    intros max h3;
+    inversion h3; subst;
+    try apply subset_refl; simpl.
+  - specialize (ast_ids_lt_trans _ _ _ h2 H9); intros hz1.
+    specialize (ast_ids_lt_trans _ _ _ h2 H10); intros hz2.
+    specialize (ast_ids_lt_add _ _ _ flag H9 hz1); intros hz3.
+    specialize (IHh1_1 hz3 _ H4).
+    specialize (lt_trans_expr _ _ _ _ _ h1_1 hz3 H4 H11); intros hz4.
+    specialize (IHh1_2 hz4 _ H5).
+    specialize (subset_close _ _ _ _ IHh1_1 H9); intros hz5.
+    specialize (subset_close1 _ _ _ _ hz5); intros hz6.
+    specialize (subset_trans _ _ _ _ _ hz6 IHh1_2 H10); auto.
+  - specialize (ast_ids_lt_trans _ _ _ h2 H9); intros hz1.
+    specialize (ast_ids_lt_trans _ _ _ h2 H10); intros hz2.
+    specialize (IHh1_1 hz1 _ H4).
+    specialize (lt_trans_expr _ _ _ _ _ h1_1 hz1 H4 H11); intros hz3.
+    specialize (IHh1_2 hz3 _ H5).
+    specialize (ast_id_bound_expr _ _ H4); intros hz4.
+    assert (hz5: get_ast_id_expr e1 < get_ast_id_expr e2); intuition.
+    specialize (subset_trans _ _ _ _ _ IHh1_1 IHh1_2 hz5); intros hz6.
+    specialize (subset_close _ _ _ _ hz6 H9); intuition.
+  - specialize (ast_ids_lt_trans _ _ _ h2 H4); intros hz1.
+    specialize (IHh1 hz1 _ H1).
+    specialize (subset_close _ _ _ _ IHh1 H4); intuition.
 Qed.
 
 
-Lemma help2: forall cks0 ls1 ls2 cks ast_id e1 e2 max1 max2 flag, 
-    ast_ids_lt cks0 ast_id ->
-    check_generator_expr cks0 e1 ls1 ->
-    check_generator_expr ls1 e2 ls2 ->
-    ast_id_inc_expr e1 max1 ->
-    ast_id_inc_expr e2 max2 -> 
-    ast_id < get_ast_id_expr e1 ->
-    ast_id < get_ast_id_expr e2 ->
-    subset ((ast_id, flag) :: ls2) cks ->
-    subset ls2 cks.
+(** it's similar to subset_expr *)
+Lemma subset_stmt: forall cks0 c cks1 max,
+    check_generator_stmt cks0 c cks1 ->
+    ast_ids_lt cks0 (get_ast_id_stmt c) -> 
+    ast_id_inc_stmt c max ->
+    subset (get_ast_id_stmt c) cks0 cks1.
+Proof.
+    intros cks0 c cks1 max h1.
+    revert max.
+    induction h1; 
+    intros max h2 h3;
+    simpl in h2; inversion h3; subst;
+    simpl.
+  - (* Sassign *)
+    specialize (ast_ids_lt_trans _ _ _ h2 H6); intros hz1.
+    specialize (subset_expr _ _ _ _ H hz1 H3); intros hz2.
+    apply subset_close with (n0 := get_ast_id_expr e); assumption.
+  - (* Sseq *)
+    specialize (ast_ids_lt_trans _ _ _ h2 H6); intros hz1.
+    specialize (IHh1_1 _ hz1 H2).
+    specialize (ast_id_max_stmt _ _ _ _ H2 h1_1 hz1); intros hz2.
+    assert (hz: max1 + 1 <= get_ast_id_stmt c2); intuition.
+    specialize (ast_ids_lt_trans0 _ _ _ hz2 hz); intros hz3.
+    specialize (IHh1_2 _ hz3 H3).
+    specialize (ast_id_bound_stmt _ _ H2); intros hz4.
+    assert (hz5: get_ast_id_stmt c1 < get_ast_id_stmt c2); intuition.
+    specialize (subset_trans _ _ _ _ _ IHh1_1 IHh1_2 hz5); intros hz6.
+    specialize (subset_close _ _ _ _ hz6 H6); auto.
+  - (* Sifthen *)
+    specialize (ast_ids_lt_trans _ _ _ h2 H7); intros hz1.
+    specialize (ast_id_max_expr _ _ _ _ H3 H hz1); intros hz2.
+    assert (hz: max1 + 1 <= get_ast_id_stmt c); intuition.
+    specialize (ast_ids_lt_trans0 _ _ _ hz2 hz); intros hz3.
+    specialize (IHh1 _ hz3 H4).
+    specialize (subset_expr _ _ _ _ H hz1 H3); intros hz4.
+    specialize (ast_id_bound_expr _ _ H3); intros hz5.
+    assert (hz6: get_ast_id_expr b < get_ast_id_stmt c); intuition.
+    specialize (subset_trans _ _ _ _ _ hz4 IHh1 hz6); intros hz7.
+    apply subset_close with (n0 := (get_ast_id_expr b)); auto.
+  - (* Swhile *)
+    specialize (ast_ids_lt_trans _ _ _ h2 H7); intros hz1.
+    specialize (ast_id_max_expr _ _ _ _ H3 H hz1); intros hz2.
+    assert (hz: max1 + 1 <= get_ast_id_stmt c); intuition.
+    specialize (ast_ids_lt_trans0 _ _ _ hz2 hz); intros hz3.
+    specialize (IHh1 _ hz3 H4).
+    specialize (subset_expr _ _ _ _ H hz1 H3); intros hz4.
+    specialize (ast_id_bound_expr _ _ H3); intros hz5.
+    assert (hz6: get_ast_id_expr b < get_ast_id_stmt c); intuition.
+    specialize (subset_trans _ _ _ _ _ hz4 IHh1 hz6); intros hz7.
+    apply subset_close with (n0 := (get_ast_id_expr b)); auto.
+Qed.
+
+
+(** 
+    help1 and help2 are just help lemmas that are used repeatedly to prove eval_expr_with_checks_correct0, 
+    so I define them as lemmas
+*)
+
+Lemma help1: forall ls0 ls1 ls2 e max n,
+    check_generator_expr ls0 e ls1 ->
+    ast_id_inc_expr e max ->
+    ast_ids_lt ls0 (get_ast_id_expr e) ->
+    n < get_ast_id_expr e ->
+    subset (max + 1) ls1 ls2 ->
+    subset (n + 1) ls0 ls2.
 Proof.
     intros.
-    specialize (fetch_ck_none _ _ H); intros h1.
-    specialize (check_update_expr _ _ _ _ _ H0 H2 h1 H4); intros h2.
-    specialize (check_update_expr _ _ _ _ _ H1 H3 h2 H5); intros h3.
-    specialize (sub_subset _ _ _ _ h3 H6); intros hz4.
-    assumption.
+    specialize (subset_expr _ _ _ _ H H1 H0); intros hz1.
+    specialize (ast_id_bound_expr _ _ H0); intros hz2.
+    assert (hz3: (get_ast_id_expr e) < (max + 1)); intuition.
+    specialize (subset_trans _ _ _ _ _ hz1 H3 hz3); intros hz4.
+    assert (hz5: n + 1 <= get_ast_id_expr e); intuition.
+    specialize (subset_close_le _ _ _ _ hz4 hz5); 
+    intuition.
+Qed.
+
+Lemma help2: forall ls0 ls1 ls2 c max n,
+    check_generator_stmt ls0 c ls1 ->
+    ast_id_inc_stmt c max ->
+    ast_ids_lt ls0 (get_ast_id_stmt c) ->
+    n < get_ast_id_stmt c ->
+    subset (max + 1) ls1 ls2 ->
+    subset (n + 1) ls0 ls2.
+Proof.
+    intros.
+    specialize (subset_stmt _ _ _ _ H H1 H0); intros hz1.
+    specialize (ast_id_bound_stmt _ _ H0); intros hz2.
+    assert (hz3: (get_ast_id_stmt c) < (max + 1)); intuition.
+    specialize (subset_trans _ _ _ _ _ hz1 H3 hz3); intros hz4.
+    assert (hz5: n + 1 <= get_ast_id_stmt c); intuition.
+    specialize (subset_close_le _ _ _ _ hz4 hz5); 
+    intuition.
 Qed.
 
 (** 
@@ -1124,112 +446,136 @@ Qed.
 *)
 Lemma eval_expr_with_checks_correct0: forall cks s e v cks1 cks0 max,
     eval_expr_with_checks cks s e v ->
-    subset cks1 cks ->
+    subset (max + 1) cks1 cks ->
     check_generator_expr cks0 e cks1 ->
     ast_ids_lt cks0 (get_ast_id_expr e) ->
     ast_id_inc_expr e max ->
     eval_expr s e v.
 Proof.
     intros cks s e v cks1 cks0 max h1.
-    generalize cks1 cks0 max.
-    clear cks1 cks0 max.
+    revert cks1 cks0 max.
     induction h1;
     intros cks1 cks0 max h2 h3 h4 h5;
     simpl in h4;
-    inversion h3; subst;
     inversion h5; subst.
   - (* Econst *) 
     constructor; auto.
   - (* Evar *)
     constructor; auto.
   - (* Ebinop *)
-    specialize (ast_ids_lt_trans _ _ _ h4 H11); intros hz1.    
-    specialize (help1 _ _ _ _ _ _ _ _ h4 H11 H13 H5 H6 H3 H4); intros hz_1.
-    specialize (help2 _ _ _ _ _ _ _ _ _ _ h4 H5 H6 H3 H4 H11 H12 h2); intros hz_2.
-    specialize (subset_trans _ _ _ hz_1 hz_2); intros hz2.
-    specialize (IHh1 _ _ _ hz2 H5 hz1 H3).
-    apply eval_Ebinop1; assumption.
-  - specialize (ast_ids_lt_trans _ _ _ h4 H11); intros hz1.
-    specialize (help1 _ _ _ _ _ _ _ _ h4 H11 H13 H5 H6 H3 H4); intros hz_1.    
-    specialize (help2 _ _ _ _ _ _ _ _ _ _ h4 H5 H6 H3 H4 H11 H12 h2); intros hz_2.
-    specialize (subset_trans _ _ _ hz_1 hz_2); intros hz2.
-    specialize (IHh1_1 _ _ _ hz2 H5 hz1 H3).
-    
-    specialize (lt_trans_expr _ _ _ _ _ H5 hz1 H3 H13); intros hz3.
-    specialize (IHh1_2 _ _ _ hz_2 H6 hz3 H4).
-    eapply eval_Ebinop2. 
-    apply IHh1_1.
-    assumption.
-  - specialize (ast_ids_lt_trans _ _ _ h4 H13); intros hz1.
-    specialize (help1 _ _ _ _ _ _ _ _ h4 H13 H15 H7 H8 H5 H6); intros hz_1.    
-    specialize (help2 _ _ _ _ _ _ _ _ _ _ h4 H7 H8 H5 H6 H13 H14 h2); intros hz_2.
-    specialize (subset_trans _ _ _ hz_1 hz_2); intros hz2.
-    specialize (IHh1_1 _ _ _ hz2 H7 hz1 H5).
-    
-    specialize (lt_trans_expr _ _ _ _ _ H7 hz1 H5 H15); intros hz_3.
-    specialize (IHh1_2 _ _ _ hz_2 H8 hz_3 H6).
-    eapply eval_Ebinop3. apply IHh1_1. apply IHh1_2.
-    inversion H9; subst.
-    { unfold subset in h2. specialize (h2 ast_id (Division_Check (Ebinop ast_id Odiv e1 e2))).
-      simpl in h2; rewrite <- beq_nat_refl in h2; intuition.
-      rewrite H in H1; inversion H1; subst.
-      econstructor. constructor. 
-      inversion H0; subst.
-      specialize (eval_expr_with_checks_unique _ _ _ _ _ h1_1 H11); intros hz3.
-      specialize (eval_expr_with_checks_unique _ _ _ _ _ h1_2 H16); intros hz4.
-      subst.
-      econstructor.
-      apply IHh1_1. apply IHh1_2.
-      assumption.
-    }
-    { unfold subset in h2. specialize (h2 ast_id No_Check).
-      simpl in h2; rewrite <- beq_nat_refl in h2; intuition.
-      rewrite H in H1; inversion H1; subst.
-      inversion H0.
-    }
-  - specialize (ast_ids_lt_trans _ _ _ h4 H14); intros hz1.
-    specialize (help1 _ _ _ _ _ _ _ _ h4 H14 H16 H9 H10 H6 H7); intros hz_1.    
-    specialize (help2 _ _ _ _ _ _ _ _ _ _ h4 H9 H10 H6 H7 H14 H15 h2); intros hz_2.
-    specialize (subset_trans _ _ _ hz_1 hz_2); intros hz2.
-    specialize (IHh1_1 _ _ _ hz2 H9 hz1 H6).
-    
-    specialize (lt_trans_expr _ _ _ _ _ H9 hz1 H6 H16); intros hz_3.
-    specialize (IHh1_2 _ _ _ hz_2 H10 hz_3 H7).
-    eapply eval_Ebinop4; auto; try assumption.
-    inversion H11; subst.
-    { unfold subset in h2. specialize (h2 ast_id (Division_Check (Ebinop ast_id Odiv e1 e2))).
-      simpl in h2; rewrite <- beq_nat_refl in h2; intuition.
-      rewrite H in H1; inversion H1; subst.
-      econstructor. constructor. 
-      inversion H0; subst. 
-      specialize (eval_expr_with_checks_unique _ _ _ _ _ h1_1 H12); intros hz3.
-      specialize (eval_expr_with_checks_unique _ _ _ _ _ h1_2 H17); intros hz4.
-      subst.
-      econstructor.
-      apply IHh1_1. apply IHh1_2.
-      assumption.
-    }
-    { econstructor. constructor.
-      assumption.
-      constructor.
-    }
+    inversion h3; subst.
+    + specialize (ast_ids_lt_trans _ _ _ h4 H8); intros hz1. 
+       specialize (ast_ids_lt_add _ _ _ flag H8 hz1); intros hz2.       
+       specialize (lt_trans_expr _ _ _ _ _ H11 hz2 H3 H10); intros hz3.
+       specialize (help1 _ _ _ _ _ _ H12 H4 hz3 H10 h2); intros hz4.       
+       specialize (IHh1 _ _ _ hz4 H11 hz2 H3).
+       constructor; assumption.
+    + specialize (ast_ids_lt_trans _ _ _ h4 H8); intros hz1.
+       specialize (lt_trans_expr _ _ _ _ _ H11 hz1 H3 H10); intros hz2.
+       specialize (help1 _ _ _ _ _ _ H12 H4 hz2 H10 h2); intros hz3.
+       specialize (IHh1 _ _ _ hz3 H11 hz1 H3).
+       constructor; assumption.
+  - inversion h3; subst.
+    + specialize (ast_ids_lt_trans _ _ _ h4 H8); intros hz1.
+       specialize (ast_ids_lt_add _ _ _ flag H8 hz1); intros hz2.
+       specialize (lt_trans_expr _ _ _ _ _ H11 hz2 H3 H10); intros hz3.
+       specialize (help1 _ _ _ _ _ _ H12 H4 hz3 H10 h2); intros hz4.
+       specialize (IHh1_1 _ _ _ hz4 H11 hz2 H3).
+       specialize (IHh1_2 _ _ _ h2 H12 hz3 H4).
+       eapply eval_Ebinop2. 
+       apply IHh1_1.
+       assumption.
+    + specialize (ast_ids_lt_trans _ _ _ h4 H8); intros hz1.
+       specialize (lt_trans_expr _ _ _ _ _ H11 hz1 H3 H10); intros hz2.
+       specialize (help1 _ _ _ _ _ _ H12 H4 hz2 H10 h2); intros hz3.
+       specialize (IHh1_1 _ _ _ hz3 H11 hz1 H3).
+       specialize (IHh1_2 _ _ _ h2 H12 hz2 H4).       
+       eapply eval_Ebinop2. 
+       apply IHh1_1.
+       assumption.
+  - inversion h3; subst.
+    + specialize (ast_ids_lt_trans _ _ _ h4 H10); intros hz1.
+       specialize (ast_ids_lt_add _ _ _ flag H10 hz1); intros hz2.
+       specialize (lt_trans_expr _ _ _ _ _ H13 hz2 H5 H12); intros hz3.
+       specialize (help1 _ _ _ _ _ _ H14 H6 hz3 H12 h2); intros hz4.
+       specialize (IHh1_1 _ _ _ hz4 H13 hz2 H5).
+       specialize (IHh1_2 _ _ _ h2 H14 hz3 H6).
+       eapply eval_Ebinop3. 
+       apply IHh1_1. apply IHh1_2.
+       assumption.
+    + specialize (ast_ids_lt_trans _ _ _ h4 H10); intros hz1.
+       specialize (lt_trans_expr _ _ _ _ _ H13 hz1 H5 H12); intros hz2.
+       specialize (help1 _ _ _ _ _ _ H14 H6 hz2 H12 h2); intros hz3.
+       specialize (IHh1_1 _ _ _ hz3 H13 hz1 H5).
+       specialize (IHh1_2 _ _ _ h2 H14 hz2 H6).
+       eapply eval_Ebinop3. 
+       apply IHh1_1. apply IHh1_2.
+       assumption.
+  - inversion h3; subst.
+    + specialize (ast_ids_lt_trans _ _ _ h4 H11); intros hz1.
+       specialize (ast_ids_lt_add _ _ _ flag H11 hz1); intros hz2.
+       specialize (lt_trans_expr _ _ _ _ _ H14 hz2 H6 H13); intros hz3.
+       specialize (help1 _ _ _ _ _ _ H15 H7 hz3 H13 h2); intros hz4.
+       specialize (IHh1_1 _ _ _ hz4 H14 hz2 H6).
+       specialize (IHh1_2 _ _ _ h2 H15 hz3 H7).
+       eapply eval_Ebinop4. 
+       apply IHh1_1. apply IHh1_2.
+       assumption. assumption.
+    + specialize (ast_ids_lt_trans _ _ _ h4 H11); intros hz1.
+       specialize (lt_trans_expr _ _ _ _ _ H14 hz1 H6 H13); intros hz2.
+       specialize (help1 _ _ _ _ _ _ H15 H7 hz2 H13 h2); intros hz3.
+       specialize (IHh1_1 _ _ _ hz3 H14 hz1 H6).
+       specialize (IHh1_2 _ _ _ h2 H15 hz2 H7).
+       eapply eval_Ebinop4. 
+       apply IHh1_1. apply IHh1_2.
+       assumption. assumption.
+  - inversion h3; subst.     
+    + specialize (ast_ids_lt_trans _ _ _ h4 H10); intros hz1.
+       specialize (ast_ids_lt_add _ _ _ flag H10 hz1); intros hz2.
+       specialize (lt_trans_expr _ _ _ _ _ H13 hz2 H5 H12); intros hz3.
+       specialize (help1 _ _ _ _ _ _ H14 H6 hz3 H12 h2); intros hz4.
+       specialize (IHh1_1 _ _ _ hz4 H13 hz2 H5).
+       specialize (IHh1_2 _ _ _ h2 H14 hz3 H6).
+       eapply eval_Ebinop4. 
+       apply IHh1_1. apply IHh1_2.
+       specialize (subset_expr _ _ _ _ H13 hz2 H5); intros hz5.
+       assert(A1: get_ast_id_expr e1 < max1 + 1).
+       specialize (ast_id_bound_expr _ _ H5); intros ha2.
+       intuition.
+       specialize (subset_trans _ _ _ _ _ hz5 hz4 A1); intros hz6.
+       unfold subset in hz6. 
+       specialize (hz6 ast_id (Some flag)).
+       unfold fetch_ck in hz6.
+       rewrite <- (beq_nat_refl ast_id) in hz6. fold fetch_ck in hz6.
+       intuition. 
+       rewrite H in H2; inversion H2.
+       assumption.
+    + specialize (ast_ids_lt_trans _ _ _ h4 H10); intros hz1.
+       specialize (lt_trans_expr _ _ _ _ _ H13 hz1 H5 H12); intros hz2.
+       specialize (help1 _ _ _ _ _ _ H14 H6 hz2 H12 h2); intros hz3.
+       specialize (IHh1_1 _ _ _ hz3 H13 hz1 H5).
+       specialize (IHh1_2 _ _ _ h2 H14 hz2 H6).
+       eapply eval_Ebinop4. 
+       apply IHh1_1. apply IHh1_2.
+       
+       destruct op; inversion H9; subst;
+       constructor; assumption.       
+       assumption.
   - (* Eunop *)
-    specialize (ast_ids_lt_trans _ _ _ h4 H6); intros hz1.
-    specialize (fetch_ck_none _ _ h4); intros h_1.
-    specialize (check_update_expr _ _ _ _ _ H2 H1 h_1 H6); intros h_2.
-    specialize (sub_subset _ _ _ _ h_2 h2); intros hz2.
-    specialize (IHh1 _ _ _ hz2 H2 hz1 H1).
+    inversion h3; subst.
+    specialize (ast_ids_lt_trans _ _ _ h4 H4); intros hz1.
+    specialize (IHh1 _ _ _ h2 H5 hz1 H1).
     econstructor; assumption.
-  - specialize (ast_ids_lt_trans _ _ _ h4 H7); intros hz1.
-    specialize (fetch_ck_none _ _ h4); intros h_1.
-    specialize (check_update_expr _ _ _ _ _ H4 H2 h_1 H7); intros h_2.
-    specialize (sub_subset _ _ _ _ h_2 h2); intros hz2.
-    specialize (IHh1 _ _ _ hz2 H4 hz1 H2).
-    
-    econstructor; auto.
+  - inversion h3; subst.
+    specialize (ast_ids_lt_trans _ _ _ h4 H5); intros hz1.
+    specialize (IHh1 _ _ _ h2 H6 hz1 H2).
+    econstructor. 
+    apply IHh1.
     assumption.
 Qed.
 
+
+(** ** eval_expr_with_checks_correct *)
 (**
     cks is checks that are generated for expression e according to the checking rules built on top of cks0, 
     then whenever e is evaluated to value v under checks cks, expression e can also be evaluated to value v 
@@ -1246,202 +592,11 @@ Theorem eval_expr_with_checks_correct: forall cks s e v cks0 max,
     eval_expr s e v.
 Proof.
     intros.
-    specialize (subset_refl cks); intros hz1.
+    specialize (subset_refl (max + 1) cks); intros hz1.
     specialize (eval_expr_with_checks_correct0 _ _ _ _ _ _ _ H hz1 H0 H1 H2).
     auto.
 Qed.
 
-(*
-(* The Proof in other way *)
-Theorem eval_expr_with_checks_correct: forall cks0 e cks max s v,
-    check_generator_expr cks0 e cks ->
-    ast_ids_lt cks0 (get_ast_id_expr e) ->
-    ast_id_inc_expr e max ->
-    eval_expr_with_checks cks s e v ->
-    eval_expr s e v.
-Proof.
-    intros cks0 e cks max s v h1.
-    generalize max s v.
-    induction h1;
-    intros max0 s0 v0 h2 h3 h4.
-  - (* Econst *)
-    inversion h4; subst.
-    constructor; auto.
-  - (* Evar *)
-    inversion h4; subst.    
-    constructor; auto.
-  - (* Ebinop *)
-    simpl in h2.
-    inversion h3; subst.
-    inversion h4; subst.
-    + specialize (ast_ids_lt_trans _ _ _ h2 H9); intros hz1.
-       specialize (eval_expr_infer1 _ _ _ _ _ _ H9 H8); intros hz2.
-       specialize (eval_expr_infer _ _ _ _ _ _ _ hz1 h1_1 h1_2 hz2); intros hz3.
-       specialize (IHh1_1 _ _ _ hz1 H4 hz3).
-       apply eval_Ebinop1. 
-       assumption.
-    + specialize (ast_ids_lt_trans _ _ _ h2 H9); intros hz1;
-       specialize (eval_expr_infer1 _ _ _ _ _ _ H9 H8); intros hz2;
-       specialize (eval_expr_infer _ _ _ _ _ _ _ hz1 h1_1 h1_2 hz2); intros hz3;
-       specialize (IHh1_1 _ _ _ hz1 H4 hz3).
-       specialize (ast_id_inc _ _ _ _ hz1 h1_1 H4); intros hz2_1;
-       assert(hz2_2: max1 + 1 <= get_ast_id_expr e2); intuition;
-       specialize (ast_ids_lt_trans0 _ _ _ hz2_1 hz2_2); intros hz2_3;
-       specialize (eval_expr_infer1 _ _ _ _ _ _ H10 H12); intros hz5;
-       specialize (IHh1_2 _ _ _ hz2_3 H5 hz5).
-       eapply eval_Ebinop2; try assumption.
-       apply IHh1_1.
-    + specialize (ast_ids_lt_trans _ _ _ h2 H9); intros hz1;
-       specialize (eval_expr_infer1 _ _ _ _ _ _ H9 H7); intros hz2;
-       specialize (eval_expr_infer _ _ _ _ _ _ _ hz1 h1_1 h1_2 hz2); intros hz3;
-       specialize (IHh1_1 _ _ _ hz1 H4 hz3).
-       specialize (ast_id_inc _ _ _ _ hz1 h1_1 H4); intros hz2_1;
-       assert(hz2_2: max1 + 1 <= get_ast_id_expr e2); intuition;
-       specialize (ast_ids_lt_trans0 _ _ _ hz2_1 hz2_2); intros hz2_3;
-       specialize (eval_expr_infer1 _ _ _ _ _ _ H10 H12); intros hz5;
-       specialize (IHh1_2 _ _ _ hz2_3 H5 hz5).
-       eapply eval_Ebinop3.
-       apply IHh1_1. apply IHh1_2.
-       inversion H; subst;
-       simpl in H13; rewrite <- beq_nat_refl in H13; inversion H13; subst.
-       { 
-         econstructor. constructor. 
-         inversion H14; subst.
-         specialize (eval_expr_with_checks_unique _ _ _ _ _ H7 H6); intros hz4.
-         specialize (eval_expr_with_checks_unique _ _ _ _ _ H12 H15); intros hz6.
-         subst.
-         econstructor.
-         apply IHh1_1. apply IHh1_2.
-         assumption.
-       }
-       { 
-         inversion H14.
-       }
-    + specialize (ast_ids_lt_trans _ _ _ h2 H9); intros hz1.
-       specialize (eval_expr_infer1 _ _ _ _ _ _ H9 H6); intros hz2;
-       specialize (eval_expr_infer _ _ _ _ _ _ _ hz1 h1_1 h1_2 hz2); intros hz3;
-       specialize (IHh1_1 _ _ _ hz1 H4 hz3).
-       specialize (ast_id_inc _ _ _ _ hz1 h1_1 H4); intros hz2_1;
-       assert(hz2_2: max1 + 1 <= get_ast_id_expr e2); intuition;
-       specialize (ast_ids_lt_trans0 _ _ _ hz2_1 hz2_2); intros hz2_3;
-       specialize (eval_expr_infer1 _ _ _ _ _ _ H10 H7); intros hz5;
-       specialize (IHh1_2 _ _ _ hz2_3 H5 hz5).
-       econstructor.
-       * apply IHh1_1.
-       * apply IHh1_2.
-       * destruct op;
-         inversion H; subst;
-         match goal with
-         | [h: check_flag (Ebinop ?ast_id Odiv ?e1 ?e2) ?check |- run_time_check eval_expr ?s0 (Ebinop ?ast_id Odiv ?e1 ?e2) true ] => idtac
-         | [h: check_flag (Ebinop ?ast_id ?op ?e1 ?e2) ?check |- run_time_check eval_expr ?s0 (Ebinop ?ast_id ?op ?e1 ?e2) true ] => 
-               econstructor; [apply H | constructor]
-         end. 
-         { simpl in H12. rewrite <- beq_nat_refl in H12. inversion H12; subst.
-           econstructor. constructor. 
-           destruct v1; destruct v2;
-           unfold eval_binop in H16; simpl in H16; intuition.
-           econstructor. apply IHh1_1. apply IHh1_2.         
-           inversion H14; subst.
-           specialize (eval_expr_with_checks_unique _ _ _ _ _ H7 H15); intros hz4.
-           inversion hz4; subst; assumption.
-         }
-         { simpl in H12. rewrite <- beq_nat_refl in H12. inversion H12; subst.
-           intuition.
-         }
-      * reflexivity.
-      * destruct v1; destruct v2;
-        destruct op;
-        match goal with
-        [h: eval_binop ?op ?v1 ?v2 = ValAbnormal -> False |- _ ] => simpl in h; intuition
-        end.
-  - (* Eunop *)
-    simpl in h2.
-    inversion h3; subst.
-    inversion h4; subst.
-    + specialize (eval_expr_infer1 _ _ _ _ _ _ H5 H6); intros hz1.
-       specialize (ast_ids_lt_trans _ _ _ h2 H5); intros hz2.
-       specialize (IHh1 _ _ _ hz2 H2 hz1).
-       econstructor. 
-       assumption.
-    + specialize (eval_expr_infer1 _ _ _ _ _ _ H5 H3); intros hz1.
-       specialize (ast_ids_lt_trans _ _ _ h2 H5); intros hz2.
-       specialize (IHh1 _ _ _ hz2 H2 hz1).
-       econstructor; auto. 
-       apply IHh1. 
-       destruct op, op0; reflexivity.
-Qed.
-*)
-
-(** these help lemmas are used to finally prove eval_stmt_with_checks_correct *)
-Lemma help3: forall cks0 cks1 cks2 c1 c2 max1 max2,
-    check_generator_stmt cks0 c1 cks1 ->
-    check_generator_stmt cks1 c2 cks2 ->
-    ast_id_inc_stmt c1 max1 ->
-    ast_id_inc_stmt c2 max2 ->
-    ast_ids_lt cks0 (get_ast_id_stmt c1) ->
-    max1 < get_ast_id_stmt c2 ->
-    subset cks1 cks2.
-Proof.
-    intros.
-    specialize (lt_trans_stmt _ _ _ _ _ H H3 H1 H4); intros hz1.
-    specialize (subset_stmt _ _ _ _ H0 hz1 H2); intuition.
-Qed.
-
-Lemma help4: forall cks0 cks1 cks2 cks3 c1 c2 max1 max2 ast_id flag,
-    check_generator_stmt cks0 c1 cks1 ->
-    check_generator_stmt cks1 c2 cks2 -> 
-    ast_id_inc_stmt c1 max1 ->
-    ast_id_inc_stmt c2 max2 ->
-    ast_id < get_ast_id_stmt c1 ->
-    ast_id < get_ast_id_stmt c2 ->
-    ast_ids_lt cks0 ast_id ->
-    subset ((ast_id, flag) :: cks2) cks3 ->
-    subset cks2 cks3.
-Proof.
-    intros.
-    specialize (fetch_ck_none _ _ H5); intros hz1.
-    specialize (check_update_stmt _ _ _ _ _ H H1 hz1 H3); intros hz2.
-    specialize (check_update_stmt _ _ _ _ _ H0 H2 hz2 H4); intros hz3.
-    specialize (sub_subset _ _ _ _ hz3 H6); intros hz4.
-    assumption.
-Qed.
-
-
-Lemma help5: forall cks0 cks1 cks2 b c max1 max2 ast_id,
-    check_generator_expr cks0 b cks1 ->
-    check_generator_stmt cks1 c cks2 ->
-    ast_id_inc_expr b max1 ->
-    ast_id_inc_stmt c max2 ->
-    max1 < get_ast_id_stmt c ->
-    ast_id < get_ast_id_expr b ->
-    ast_ids_lt cks0 ast_id ->
-    subset cks1 cks2.
-Proof.
-    intros.
-    specialize (ast_ids_lt_trans _ _ _ H5 H4); intros hz1.
-    specialize (lt_trans_expr _ _ _ _ _ H hz1 H1 H3); intros hz2.
-    specialize (subset_stmt _ _ _ _ H0 hz2 H2); intros hz5.
-    assumption.
-Qed.
-
-Lemma help6: forall cks0 cks1 cks2 cks3 b c max1 max2 ast_id flag,
-    check_generator_expr cks0 b cks1 ->
-    check_generator_stmt cks1 c cks2 ->
-    ast_id_inc_expr b max1 ->
-    ast_id_inc_stmt c max2 ->
-    ast_id < get_ast_id_expr b ->
-    ast_id < get_ast_id_stmt c -> 
-    ast_ids_lt cks0 ast_id ->
-    subset ((ast_id, flag) :: cks2) cks3 ->
-    subset cks2 cks3.
-Proof.
-    intros.
-    specialize (fetch_ck_none _ _ H5); intros hz_1.
-    specialize (check_update_expr _ _ _ _ _ H H1 hz_1 H3); intros hz_2.
-    specialize (check_update_stmt _ _ _ _ _ H0 H2 hz_2 H4); intros hz_3.
-    specialize (sub_subset _ _ _ _ hz_3 H6); intros hz_4.
-    assumption.
-Qed.
 
 (** 
     Because we cannot prove eval_stmt_with_checks_correct directly, so 
@@ -1450,7 +605,7 @@ Qed.
 *)
 Theorem eval_stmt_with_checks_correct_0: forall cks s c s' cks1 cks0 max,
     eval_stmt_with_checks cks s c s' ->
-    subset cks1 cks ->
+    subset (max + 1) cks1 cks ->
     check_generator_stmt cks0 c cks1 ->
     ast_ids_lt cks0 (get_ast_id_stmt c) ->
     ast_id_inc_stmt c max ->
@@ -1464,101 +619,75 @@ Proof.
     simpl in h4; inversion h3; inversion h5; subst.
   - (* Sassign *)
     specialize (ast_ids_lt_trans _ _ _ h4 H12); intros hz1.
-    specialize (fetch_ck_none _ _ h4); intros h_1.
-    specialize (check_update_expr _ _ _ _ _ H5 H9 h_1 H12); intros h_2.
-    specialize (sub_subset _ _ _ _ h_2 h2); intros hz2.
-    specialize (eval_expr_with_checks_correct0 _ _ _ _ _ _ _ H hz2 H5 hz1 H9); intros hz3.
+    specialize (eval_expr_with_checks_correct0 _ _ _ _ _ _ _ H h2 H5 hz1 H9); intros hz2.
     constructor;
     assumption.
   - specialize (ast_ids_lt_trans _ _ _ h4 H13); intros hz1.
-    specialize (fetch_ck_none _ _ h4); intros h_1.
-    specialize (check_update_expr _ _ _ _ _ H6 H10 h_1 H13); intros h_2.
-    specialize (sub_subset _ _ _ _ h_2 h2); intros hz2.
-    specialize (eval_expr_with_checks_correct0 _ _ _ _ _ _ _ H hz2 H6 hz1 H10); intros hz3.
+    specialize (eval_expr_with_checks_correct0 _ _ _ _ _ _ _ H h2 H6 hz1 H10); intros hz2.
     econstructor.
-    apply hz3.
+    apply hz2.
     assumption.
   - (* Sseq *)
     specialize (ast_ids_lt_trans _ _ _ h4 H13); intros hz1.
-    specialize (help3 _ _ _ _ _ _ _ H4 H5 H9 H10 hz1 H16); intros hz_1.
-    specialize (help4 _ _ _ _ _ _ _ _ _ _ H4 H5 H9 H10 H13 H15 h4 h2); intros hz_2.
-    specialize (subset_trans _ _ _ hz_1 hz_2); intros hz2.
-    specialize (IHh1 _ _ _ hz2 H4 hz1 H9).
+    specialize (lt_trans_stmt _ _ _ _ _ H4 hz1 H9 H16); intros hz2.
+    specialize (help2 _ _ _ _ _ _ H5 H10 hz2 H16 h2); intros hz3.
+    specialize (IHh1 _ _ _ hz3 H4 hz1 H9).
     constructor; assumption.
   - specialize (ast_ids_lt_trans _ _ _ h4 H13); intros hz1.
-    specialize (help3 _ _ _ _ _ _ _ H4 H5 H9 H10 hz1 H16); intros hz_1.
-    specialize (help4 _ _ _ _ _ _ _ _ _ _ H4 H5 H9 H10 H13 H15 h4 h2); intros hz_2.
-    specialize (subset_trans _ _ _ hz_1 hz_2); intros hz2.
-    specialize (IHh1_1 _ _ _ hz2 H4 hz1 H9).
-
-    specialize (lt_trans_stmt _ _ _ _ _ H4 hz1 H9 H16); intros hz3.
-    specialize (IHh1_2 _ _ _ hz_2 H5 hz3 H10).
+    specialize (lt_trans_stmt _ _ _ _ _ H4 hz1 H9 H16); intros hz2.
+    specialize (help2 _ _ _ _ _ _ H5 H10 hz2 H16 h2); intros hz3.
+    specialize (IHh1_1 _ _ _ hz3 H4 hz1 H9).
+    specialize (IHh1_2 _ _ _ h2 H5 hz2 H10).
     econstructor.
     apply IHh1_1.
     assumption.
   - (* Sifthen *)
     specialize (ast_ids_lt_trans _ _ _ h4 H14); intros hz1.
-    specialize (help5 _ _ _ _ _ _ _ _ H5 H6 H10 H11 H17 H14 h4); intros hz_1.
-    specialize (help6 _ _ _ _ _ _ _ _ _ _ H5 H6 H10 H11 H14 H16 h4 h2); intros hz_2.
-    specialize (subset_trans _ _ _ hz_1 hz_2); intros hz2.
-    specialize (eval_expr_with_checks_correct0 _ _ _ _ _ _ _ H hz2 H5 hz1 H10); intros hz3.
+    specialize (lt_trans_expr _ _ _ _ _ H5 hz1 H10 H17); intros hz2.
+    specialize (help2 _ _ _ _ _ _ H6 H11 hz2 H17 h2); intros hz3.
+    specialize (eval_expr_with_checks_correct0 _ _ _ _ _ _ _ H hz3 H5 hz1 H10); intros hz4.
     constructor; 
-    assumption.
-  - specialize (ast_ids_lt_trans _ _ _ h4 H14); intros hz1.
-    specialize (help6 _ _ _ _ _ _ _ _ _ _ H5 H6 H10 H11 H14 H16 h4 h2); intros hz2.
-    specialize (lt_trans_expr _ _ _ _ _ H5 hz1 H10 H17); intros hz3.
-    specialize (IHh1 _ _ _ hz2 H6 hz3 H11).
-    econstructor; try assumption.
-    
-    specialize (help5 _ _ _ _ _ _ _ _ H5 H6 H10 H11 H17 H14 h4); intros hz4.
-    specialize (subset_trans _ _ _ hz4 hz2); intros hz5.
-    specialize (eval_expr_with_checks_correct0 _ _ _ _ _ _ _ H hz5 H5 hz1 H10); intros hz6.
-    assumption. 
-  - apply eval_Sifthen_False.
-    specialize (ast_ids_lt_trans _ _ _ h4 H14); intros hz1.
-    specialize (help5 _ _ _ _ _ _ _ _ H5 H6 H10 H11 H17 H14 h4); intros hz_1.
-    specialize (help6 _ _ _ _ _ _ _ _ _ _ H5 H6 H10 H11 H14 H16 h4 h2); intros hz_2.
-    specialize (subset_trans _ _ _ hz_1 hz_2); intros hz2.
-    specialize (eval_expr_with_checks_correct0 _ _ _ _ _ _ _ H hz2 H5 hz1 H10); intros hz3.
-    assumption.
-  - (* Swhile *)
-    specialize (ast_ids_lt_trans _ _ _ h4 H14); intros hz1.
-    specialize (help5 _ _ _ _ _ _ _ _ H5 H6 H10 H11 H17 H14 h4); intros hz_1.
-    specialize (help6 _ _ _ _ _ _ _ _ _ _ H5 H6 H10 H11 H14 H16 h4 h2); intros hz_2.
-    specialize (subset_trans _ _ _ hz_1 hz_2); intros hz2.
-    specialize (eval_expr_with_checks_correct0 _ _ _ _ _ _ _ H hz2 H5 hz1 H10); intros hz3.
-    constructor; 
-    assumption.    
-  - specialize (ast_ids_lt_trans _ _ _ h4 H14); intros hz1.
-    specialize (help6 _ _ _ _ _ _ _ _ _ _ H5 H6 H10 H11 H14 H16 h4 h2); intros hz2.
-    specialize (lt_trans_expr _ _ _ _ _ H5 hz1 H10 H17); intros hz3.
-    specialize (IHh1 _ _ _ hz2 H6 hz3 H11). 
-    apply eval_Swhile_True1; try assumption.
-    specialize (help5 _ _ _ _ _ _ _ _ H5 H6 H10 H11 H17 H14 h4); intros hz4.
-    specialize (subset_trans _ _ _ hz4 hz2); intros hz5.
-    specialize (eval_expr_with_checks_correct0 _ _ _ _ _ _ _ H hz5 H5 hz1 H10); intros hz6.
     assumption.
   - specialize (ast_ids_lt_trans _ _ _ h4 H14); intros hz1.
     specialize (lt_trans_expr _ _ _ _ _ H5 hz1 H10 H17); intros hz2.
-    specialize (help6 _ _ _ _ _ _ _ _ _ _ H5 H6 H10 H11 H14 H16 h4 h2); intros hz3.
-    specialize (IHh1_1 _ _ _ hz3 H6 hz2 H11).
-    specialize (IHh1_2 _ _ _ h2 h3 h4 h5).
-    eapply eval_Swhile_True2.
-    specialize (help5 _ _ _ _ _ _ _ _ H5 H6 H10 H11 H17 H14 h4); intros hz4.
-    specialize (subset_trans _ _ _ hz4 hz3); intros hz5.
-    specialize (eval_expr_with_checks_correct0 _ _ _ _ _ _ _ H hz5 H5 hz1 H10); intros hz6.
-    assumption.
-    apply IHh1_1.
-    assumption.
-  - apply eval_Swhile_False.
+    specialize (help2 _ _ _ _ _ _ H6 H11 hz2 H17 h2); intros hz3.
+    specialize (eval_expr_with_checks_correct0 _ _ _ _ _ _ _ H hz3 H5 hz1 H10); intros hz4.
+    specialize (IHh1 _ _ _ h2 H6 hz2 H11).
+    econstructor; try assumption. 
+  - specialize (ast_ids_lt_trans _ _ _ h4 H14); intros hz1.
+    specialize (lt_trans_expr _ _ _ _ _ H5 hz1 H10 H17); intros hz2.
+    specialize (help2 _ _ _ _ _ _ H6 H11 hz2 H17 h2); intros hz3.
+    specialize (eval_expr_with_checks_correct0 _ _ _ _ _ _ _ H hz3 H5 hz1 H10); intros hz4.
+    apply eval_Sifthen_False; assumption.
+  - (* Swhile *)
     specialize (ast_ids_lt_trans _ _ _ h4 H14); intros hz1.
-    specialize (help5 _ _ _ _ _ _ _ _ H5 H6 H10 H11 H17 H14 h4); intros hz_1.
-    specialize (help6 _ _ _ _ _ _ _ _ _ _ H5 H6 H10 H11 H14 H16 h4 h2); intros hz_2.    
-    specialize (subset_trans _ _ _ hz_1 hz_2); intros hz2.
-    specialize (eval_expr_with_checks_correct0 _ _ _ _ _ _ _ H hz2 H5 hz1 H10); intros hz3.
-    assumption.
+    specialize (lt_trans_expr _ _ _ _ _ H5 hz1 H10 H17); intros hz2.
+    specialize (help2 _ _ _ _ _ _ H6 H11 hz2 H17 h2); intros hz3.
+    specialize (eval_expr_with_checks_correct0 _ _ _ _ _ _ _ H hz3 H5 hz1 H10); intros hz4.
+    constructor; 
+    assumption.   
+  - specialize (ast_ids_lt_trans _ _ _ h4 H14); intros hz1.
+    specialize (lt_trans_expr _ _ _ _ _ H5 hz1 H10 H17); intros hz2.
+    specialize (help2 _ _ _ _ _ _ H6 H11 hz2 H17 h2); intros hz3.
+    specialize (eval_expr_with_checks_correct0 _ _ _ _ _ _ _ H hz3 H5 hz1 H10); intros hz4.
+    specialize (IHh1 _ _ _ h2 H6 hz2 H11).
+    eapply eval_Swhile_True1; try assumption.
+  - specialize (ast_ids_lt_trans _ _ _ h4 H14); intros hz1.
+    specialize (lt_trans_expr _ _ _ _ _ H5 hz1 H10 H17); intros hz2.
+    specialize (help2 _ _ _ _ _ _ H6 H11 hz2 H17 h2); intros hz3.
+    specialize (eval_expr_with_checks_correct0 _ _ _ _ _ _ _ H hz3 H5 hz1 H10); intros hz4.
+    specialize (IHh1_1 _ _ _ h2 H6 hz2 H11).
+    specialize (IHh1_2 _ _ _ h2 h3 h4 h5).
+    eapply eval_Swhile_True2; auto.
+    apply IHh1_1. apply IHh1_2.
+  - specialize (ast_ids_lt_trans _ _ _ h4 H14); intros hz1.
+    specialize (lt_trans_expr _ _ _ _ _ H5 hz1 H10 H17); intros hz2.
+    specialize (help2 _ _ _ _ _ _ H6 H11 hz2 H17 h2); intros hz3.
+    specialize (eval_expr_with_checks_correct0 _ _ _ _ _ _ _ H hz3 H5 hz1 H10); intros hz4.
+    eapply eval_Swhile_False; auto.
 Qed.
 
+(** ** eval_stmt_with_checks_correct *)
 (**
     cks is checks that are generated for statement c according to the checking rules built on top of cks0, 
     then whenever c is evaluated to a state s' under checks cks, statement c can also be evaluated to state s' 
@@ -1575,7 +704,7 @@ Theorem eval_stmt_with_checks_correct: forall cks s c s' cks0 max,
     eval_stmt s c s'.
 Proof.
     intros.
-    specialize (subset_refl cks); intros hz1.
+    specialize (subset_refl (max + 1) cks); intros hz1.
     specialize (eval_stmt_with_checks_correct_0 _ _ _ _ _ _ _ H hz1 H0 H1 H2).
     auto.
 Qed.
