language_formal/spark2014_semantics/wellformedness.v
@@ -40,15 +40,14 @@ Definition binop_type (op: binary_operation) (x y: typ): option typ :=
 (** ** Well-typed expressions *)
 (**
    - general type check for expressions;
-   - all variables used in expression should be in mode _in_ or _in/out_; 
 *)
 Inductive well_typed_expr: symtb -> expr -> typ -> Prop :=
     | WT_Econst_Int: forall ast_id n tb,
         well_typed_expr tb (Econst ast_id (Ointconst n)) Tint
     | WT_Econst_Bool: forall ast_id b tb,
         well_typed_expr tb (Econst ast_id (Oboolconst b)) Tbool
-    | WT_Evar: forall ast_id x tb t,
-        lookup x tb = Some (In, t) ->  (* the 'out' variables can never be read *)    
+    | WT_Evar: forall ast_id x tb m t,
+        lookup x tb = Some (m, t) ->  
         well_typed_expr tb (Evar ast_id x) t
     | WT_Ebinop: forall ast_id tb op e1 e2 t t1,
         well_typed_expr tb e1 t ->
@@ -62,13 +61,11 @@ Inductive well_typed_expr: symtb -> expr -> typ -> Prop :=
 
 (** ** Well-typed commands *)
 (**
-   two kinds of type checking:
-   - general type checking;
-   - _in/out_ mode checking (for variables that are updated by assignments, their mode should be _out_ or _in\out_);
+    - general type checking;
 *)
 Inductive well_typed_stmt: symtb -> stmt  -> Prop :=
-    | WT_Sassign: forall ast_id tb x e t,
-        lookup x tb = Some (Out, t) ->
+    | WT_Sassign: forall ast_id tb x e m t,
+        lookup x tb = Some (m, t) ->
         well_typed_expr tb e t ->
         well_typed_stmt tb ((Sassign ast_id x e))
     | WT_Sseq: forall ast_id c1 c2 tb,
@@ -97,26 +94,27 @@ Inductive init_mode: Type :=
     | Init: init_mode
     | Uninit: init_mode.
 
-Definition initializationState: Type := list (idnum * init_mode).
+(** map from variable to its initialization state and in/out mode *)
+Definition mode_map: Type := list (idnum * (init_mode * mode)).
 
 (** basic functions for fetching and updating the variable's initialization state *)
-Function fetch2 (x : idnum) (s : initializationState): option init_mode := 
+Function fetch2 (x : idnum) (s : mode_map): option (init_mode * mode) := 
     match s with 
-    | (y, imode) :: s' =>
+    | (y, m) :: s' =>
       if beq_nat x y then
-        Some imode
+        Some m
       else fetch2 x s' 
     | nil => None
     end.
 
-Function update2 (s: initializationState) (x : idnum) (v: init_mode): option initializationState := 
+Function update2 (s: mode_map) (x : idnum) (m: (init_mode * mode)): option mode_map := 
     match s with 
-    | (y, imode) :: s' => 
+    | (y, m0) :: s' => 
       if beq_nat x y then 
-        Some ((y,v)::s') 
+        Some ((y,m)::s') 
       else 
-        match update2 s' x v with
-        | Some s'' => Some ((y, imode)::s'')
+        match update2 s' x m with
+        | Some s'' => Some ((y, m0)::s'')
         | None => None
         end
    | nil => None
@@ -124,41 +122,25 @@ Function update2 (s: initializationState) (x : idnum) (v: init_mode): option ini
 
 (** ** Well-defined expressions *)
 (**
-    all referenced variables are initialized 
+   - all referenced variables are initialized 
+   - all variables used in expression should be in mode _in_ or _in/out_; 
 *)
-Inductive well_defined_expr: initializationState -> expr -> Prop :=
-    | WD_Econst_Int: forall ast_id s n,
-        well_defined_expr s (Econst ast_id (Ointconst n))
-    | WD_Econst_Bool: forall ast_id s b,
-        well_defined_expr s (Econst ast_id (Oboolconst b))
-    | WD_Evar: forall ast_id x s,
-        fetch2 x s = Some Init ->
-        well_defined_expr s (Evar ast_id x)
-    | WD_Ebinop: forall ast_id s op e1 e2,
-        well_defined_expr s e1 ->
-        well_defined_expr s e2 ->
-        well_defined_expr s (Ebinop ast_id op e1 e2)
-    | WD_Eunop: forall ast_id s op e,
-        well_defined_expr s e ->
-        well_defined_expr s (Eunop ast_id op e). 
+Inductive well_defined_expr: mode_map -> expr -> Prop :=
+    | WD_Econst_Int: forall ast_id m n,
+        well_defined_expr m (Econst ast_id (Ointconst n))
+    | WD_Econst_Bool: forall ast_id m b,
+        well_defined_expr m (Econst ast_id (Oboolconst b))
+    | WD_Evar: forall ast_id x m,
+        fetch2 x m = Some (Init, In) \/ fetch2 x m = Some (Init, InOut) ->
+        well_defined_expr m (Evar ast_id x)
+    | WD_Ebinop: forall ast_id m op e1 e2,
+        well_defined_expr m e1 ->
+        well_defined_expr m e2 ->
+        well_defined_expr m (Ebinop ast_id op e1 e2)
+    | WD_Eunop: forall ast_id m op e,
+        well_defined_expr m e ->
+        well_defined_expr m (Eunop ast_id op e). 
 
-(*
-Inductive well_defined_expr: stack -> expr -> Prop :=
-    | WD_Econst_Int: forall ast_id s n,
-        well_defined_expr s (Econst ast_id (Ointconst n))
-    | WD_Econst_Bool: forall ast_id s b,
-        well_defined_expr s (Econst ast_id (Oboolconst b))
-    | WD_Evar: forall ast_id x v s,
-        fetch x s = Some v ->
-        well_defined_expr s (Evar ast_id x)
-    | WD_Ebinop: forall ast_id s op e1 e2,
-        well_defined_expr s e1 ->
-        well_defined_expr s e2 ->
-        well_defined_expr s (Ebinop ast_id op e1 e2)
-    | WD_Eunop: forall ast_id s op e,
-        well_defined_expr s e ->
-        well_defined_expr s (Eunop ast_id op e). 
-*)
 
 (** ** Well-defined commands *)
 (** 
@@ -168,36 +150,38 @@ Inductive well_defined_expr: stack -> expr -> Prop :=
     are initialized or not;
     For conditional and while loop commands, their final initialization state are the intersection 
     of the resulting initialization states from both branches;
+   - _in/out_ mode checking (for variables that are updated by assignments, their mode should be _out_ or _in\out_);
 *)
-Inductive well_defined_stmt: initializationState -> stmt -> initializationState -> Prop :=
-    | WD_Sassign: forall ast_id s s' x e,
-        well_defined_expr s e ->
-        update2 s x Init = Some s' ->
-        well_defined_stmt s (Sassign ast_id x e) s'
-    | WD_Sseq: forall ast_id c1 c2 s s' s'',
-        well_defined_stmt s c1 s' ->
-        well_defined_stmt s' c2 s'' ->
-        well_defined_stmt s (Sseq ast_id c1 c2) s''
-    | WD_Sifthen: forall ast_id s s' b c,
-        well_defined_expr s b ->
-        well_defined_stmt s c s' ->
-        well_defined_stmt s (Sifthen ast_id b c) s
-    | WD_Swhile: forall ast_id s s' b c,
-        well_defined_expr s b ->
-        well_defined_stmt s c s' ->
-        well_defined_stmt s (Swhile ast_id b c) s.
+Inductive well_defined_stmt: mode_map -> stmt -> mode_map -> Prop :=
+    | WD_Sassign: forall ast_id m m' i x e,
+        well_defined_expr m e ->
+        fetch2 x m = Some (i, Out) \/ fetch2 x m = Some (i, InOut) ->
+        update2 m x (Init, InOut) = Some m' ->
+        well_defined_stmt m (Sassign ast_id x e) m'
+    | WD_Sseq: forall ast_id c1 c2 m m' m'',
+        well_defined_stmt m c1 m' ->
+        well_defined_stmt m' c2 m'' ->
+        well_defined_stmt m (Sseq ast_id c1 c2) m''
+    | WD_Sifthen: forall ast_id m m' b c,
+        well_defined_expr m b ->
+        well_defined_stmt m c m' ->
+        well_defined_stmt m (Sifthen ast_id b c) m
+    | WD_Swhile: forall ast_id m m' b c,
+        well_defined_expr m b ->
+        well_defined_stmt m c m' ->
+        well_defined_stmt m (Swhile ast_id b c) m.
 
 (** ** Lemmas for fetching and updating initialization state *)
-Lemma update2_fetch2: forall istate x m istate',
-    update2 istate x m = Some istate' ->
-    exists m0, fetch2 x istate = Some m0.
+Lemma update2_fetch2: forall s x m s',
+    update2 s x m = Some s' ->
+    exists m0, fetch2 x s = Some m0.
 Proof.
-    intros istate x m.
-    functional induction (update2 istate x m);
-    intros istate' h1.
+    intros s x m.
+    functional induction (update2 s x m);
+    intros s'0 h1.
   - unfold fetch2.
     rewrite e0.
-    exists imode; auto.
+    exists m0; auto.
   - unfold fetch2.
     rewrite e0.
     fold fetch2.
@@ -206,34 +190,34 @@ Proof.
   - inversion h1.
 Qed.
 
-Lemma fetch2_update2: forall x istate m0 m,
-    fetch2 x istate = Some m0 ->
-    exists istate', update2 istate x m = Some istate'.
+Lemma fetch2_update2: forall x s m0 m,
+    fetch2 x s = Some m0 ->
+    exists s', update2 s x m = Some s'.
 Proof.
-    intros x istate.
-    functional induction (fetch2 x istate);
-    intros m0 m h1.
+    intros x s.
+    functional induction (fetch2 x s);
+    intros m0 m1 h1.
   - unfold update2.
     rewrite e0.
-    exists ((y, m) :: s'); auto.
+    exists ((y, m1) :: s'); auto.
   - unfold update2. 
     rewrite e0.
     fold update2.
-    specialize (IHo _ m h1).
+    specialize (IHo _ m1 h1).
     inversion IHo.
     rewrite H.
-    exists ((y, imode) :: x0); auto.
+    exists ((y, m) :: x0); auto.
   - inversion h1.
 Qed.
 
-Lemma update2_in: forall istate x m istate' y m',
-    update2 istate x m = Some istate' ->
-    fetch2 y istate = Some m' ->
-    (fetch2 y istate' = Some m) \/ (fetch2 y istate' = Some m').
+Lemma update2_in: forall s x m s' y m',
+    update2 s x m = Some s' ->
+    fetch2 y s = Some m' ->
+    (fetch2 y s' = Some m) \/ (fetch2 y s' = Some m').
 Proof.
-    intros istate x m.
-    functional induction (update2 istate x m);
-    intros istate' y0 m' h1 h2.
+    intros s x m.
+    functional induction (update2 s x m);
+    intros s'0 y0 m' h1 h2.
   - inversion h1; subst.
     unfold fetch2.
     unfold fetch2 in h2.
@@ -255,14 +239,14 @@ Proof.
   - inversion h1.
 Qed.
 
-Lemma update2_in1: forall istate x m istate' y m',
-    update2 istate x m = Some istate' ->
-    fetch2 y istate' = Some m' ->
-    (y = x /\ m' = m) \/ (y <> x /\ fetch2 y istate = Some m').
+Lemma update2_in1: forall s x m s' y m',
+    update2 s x m = Some s' ->
+    fetch2 y s' = Some m' ->
+    (y = x /\ m' = m) \/ (y <> x /\ fetch2 y s = Some m').
 Proof.
-    intros istate x m.
-    functional induction (update2 istate x m);
-    intros istate' y0 m' h1 h2.
+    intros s x m.
+    functional induction (update2 s x m);
+    intros s'0 y0 m' h1 h2.
   - inversion h1; subst.
     unfold fetch2.
     unfold fetch2 in h2.
@@ -300,13 +284,13 @@ Proof.
   - inversion h1.  
 Qed.
 
-Lemma update2_fetch2_new: forall istate x m istate',
-    update2 istate x m = Some istate' ->
-    fetch2 x istate' = Some m.
+Lemma update2_fetch2_new: forall s x m s',
+    update2 s x m = Some s' ->
+    fetch2 x s' = Some m.
 Proof.
-    intros istate x m.
-    functional induction (update2 istate x m);
-    intros istate' h1.
+    intros s x m.
+    functional induction (update2 s x m);
+    intros s'0 h1.
   - inversion h1; subst.
     unfold fetch2.
     destruct (beq_nat x y).
@@ -323,14 +307,14 @@ Proof.
   - inversion h1.    
 Qed.
 
-Lemma update2_fetch2_old: forall istate x m istate' y,
-    update2 istate x m = Some istate' ->
+Lemma update2_fetch2_old: forall s x m s' y,
+    update2 s x m = Some s' ->
     y <> x ->
-    fetch2 y istate' = fetch2 y istate.
+    fetch2 y s' = fetch2 y s.
 Proof.
-    intros istate x m.
-    functional induction (update2 istate x m);
-    intros istate' y0 h1 h2.
+    intros s x m.
+    functional induction (update2 s x m);
+    intros s'0 y0 h1 h2.
   - inversion h1; subst.
     apply beq_nat_true in e0.
     subst.
@@ -350,162 +334,73 @@ Proof.
   - inversion h1.    
 Qed.
 
-(** ** Mapping from stack to initialization state *)
+(** ** Constructing mode map mapping from variable id to (initialization state * in/out mode)  *)
 (** 
    for any variable in stack, if it has a defined value then it has an initialized state,
    otherwise, it's uninitialized;
 *)
-Inductive initializationMap: stack -> initializationState -> Prop :=
-    | IEmpty: initializationMap nil nil 
-    | IList0: forall s ilist x v,
-        v <> Vundef ->
-        initializationMap s ilist ->
-        initializationMap ((x, v)::s) ((x, Init)::ilist)
-    | IList1: forall s ilist x v,
-        v = Vundef ->
-        initializationMap s ilist ->
-        initializationMap ((x, v)::s) ((x, Uninit)::ilist).
+Inductive mode_mapping: symtb -> stack -> (mode_map) -> Prop :=
+    | M_Empty: mode_mapping nil nil nil
+    | M_Bool: forall tb s x m b ls,
+          mode_mapping tb s ls ->
+          mode_mapping ((x, (m, Tbool)) :: tb) ((x, (Value (Bool b))) :: s) ((x, (Init, m)) :: ls)
+    | M_Int: forall tb s x m v ls,
+          mode_mapping tb s ls ->
+          mode_mapping ((x, (m, Tint)) :: tb) ((x, (Value (Int v))) :: s) ((x, (Init, m)) :: ls)
+    | M_UndefBool: forall tb s x m ls,
+          mode_mapping tb s ls ->
+          mode_mapping ((x, (m, Tbool)) :: tb) ((x, Vundef) :: s) ((x, (Uninit, m)) :: ls)
+    | M_UndefInt: forall tb s x m ls,
+          mode_mapping tb s ls ->
+          mode_mapping ((x, (m, Tint)) :: tb) ((x, Vundef) :: s) ((x, (Uninit, m)) :: ls).
 
-(** some useful lemmas *)
-(** 
-    'istate' is an initialization state map (from variable to initialization mode: Init or Uninit) that's constructed
-    from the stack 's' (mapping from variable to defined value or undefined value);
-    when we fetch a variable 'x' from stack 's', if it returns some value 'v', then the result should be the 'Init' mode 
-    when we fetch it from the corresponding initialization state map 'istate';
-*)
-Lemma initializationMap_consistent1: forall s istate x v,
-    initializationMap s istate -> 
-    fetch x s = Some v -> 
-    fetch2 x istate = Some Init.
+Lemma mode_map_exists: forall tb s,
+    type_check_stack tb s ->
+    exists m, mode_mapping tb s m.
 Proof.
-    intros s istate x v h1 h2.
-    induction h1.
-      + inversion h2.
-      + unfold fetch in h2. 
-         unfold fetch2.
-         destruct (beq_nat x x0); auto.
-      + unfold fetch in h2.
-         unfold fetch2.
-         destruct (beq_nat x x0);
-         auto.
-         destruct v0.
-         inversion H.
-         inversion h2.
+    intros.
+    induction H;
+    [ exists nil; constructor | | | | ];
+    inversion IHtype_check_stack;
+    [exists ((x, (Init, m)) :: x0) | exists ((x, (Init, m)) :: x0) | 
+     exists ((x, (Uninit, m)) :: x0) | exists ((x, (Uninit, m)) :: x0)
+    ]; constructor; assumption.
 Qed.
 
-(** the reverse is the same *)
-Lemma initializationMap_consistent2: forall s istate x,
-    initializationMap s istate ->
-    fetch2 x istate = Some Init -> 
+Lemma fetch_exists: forall tb s m x y,
+    mode_mapping tb s m ->
+    fetch2 x m = Some (Init, y) ->
     exists v, fetch x s = Some v.
-Proof.
-    intros s istate x h1 h2.
+Proof. 
+    intros tb s m x y h1 h2.
     induction h1.
-      + inversion h2.
-      + unfold fetch2 in h2. 
-         unfold fetch.
-         destruct (beq_nat x x0); auto.
-         destruct v.
-         exists v; auto.
-         intuition.
-      + unfold fetch2 in h2.
-         unfold fetch.
-         destruct (beq_nat x x0); auto.
-         destruct v.
-         exists v; auto.
-         inversion h2.    
-Qed.
-
-(** for any stack s, we can only compute one initialization state Map from s *)
-Lemma initializationMap_unique: forall s istate istate',
-    initializationMap s istate ->
-    initializationMap s istate' ->
-    istate = istate'.
-Proof.
-    intros s istate istate' h1.
-    generalize istate'. clear istate'.
-    induction h1;
-    intros istate' h2.
   - inversion h2.
-    auto.
-  - inversion h2; subst.
-    specialize (IHh1 _ H5).
-    subst. auto.
-    intuition.
-  - inversion h2; subst.
-    intuition.
-    specialize (IHh1 _ H5).
-    subst.
-    auto.
+  - unfold fetch2 in h2.
+    unfold fetch.
+    destruct (beq_nat x x0).
+    exists (Bool b); reflexivity.
+    fold fetch. fold fetch2 in h2.
+    apply IHh1; assumption.
+  - unfold fetch2 in h2.
+    unfold fetch.
+    destruct (beq_nat x x0).
+    exists (Int v); reflexivity.
+    fold fetch. fold fetch2 in h2.
+    apply IHh1; assumption.
+  - unfold fetch2 in h2.
+    unfold fetch.
+    destruct (beq_nat x x0).
+    inversion h2.
+    fold fetch. fold fetch2 in h2.
+    apply IHh1; assumption.
+  - unfold fetch2 in h2.
+    unfold fetch.
+    destruct (beq_nat x x0).
+    inversion h2.
+    fold fetch. fold fetch2 in h2.
+    apply IHh1; assumption.
 Qed.
 
-(** when we update the stack s with x by a new value v, the initialization state map istate'1 computed
-     from s1 should be equal to the initialization state istate1 that update istate with x by Init directly;
-*)
-Lemma update_consis: forall s istate x v s1 istate1 istate'1,
-    initializationMap s istate -> 
-    update s x (Value v) = Some s1 ->
-    update2 istate x Init = Some istate1 ->
-    initializationMap s1 istate'1 ->
-    istate1 = istate'1.
-Proof.
-    intros s istate x v s1 istate1 istate'1 h1.
-    generalize x v s1 istate1 istate'1.
-    induction h1; intros.
-  - inversion H.
-  - unfold update in H0.
-    unfold update2 in H1.
-    destruct (beq_nat x1 x0).
-    + inversion H0; subst.
-       inversion H1; subst.
-       inversion H2; subst.
-       * specialize (initializationMap_unique _ _ _ h1 H8); intros hz1.
-         subst.
-         auto.
-       * inversion H7.
-    + fold update in H0.
-       fold update2 in H1.
-       remember (update s x1 (Value v1)) as eq1.
-       remember (update2 ilist x1 Init) as eq2.
-       destruct eq1; destruct eq2.
-       * inversion H0; subst; clear H0.
-         inversion H1; subst; clear H1.
-         symmetry in Heqeq1. 
-         symmetry in Heqeq2.
-         inversion H2; subst.
-         specialize (IHh1 _ _ _ _ _ Heqeq1 Heqeq2 H6).
-         subst. auto.
-         intuition.
-       * inversion H1.
-       * inversion H0.
-       * inversion H0.
-  - unfold update in H0.
-    unfold update2 in H1.
-    destruct (beq_nat x1 x0).
-    + inversion H0; subst.
-       inversion H1; subst.
-       inversion H2; subst.
-       * specialize (initializationMap_unique _ _ _ h1 H7); intros hz1.
-         subst.
-         auto.
-       * inversion H6.
-    + fold update in H0.
-       fold update2 in H1.
-       remember (update s x1 (Value v1)) as eq1.
-       remember (update2 ilist x1 Init) as eq2.
-       destruct eq1; destruct eq2.
-       * inversion H0; subst; clear H0.
-         inversion H1; subst; clear H1.
-         symmetry in Heqeq1. 
-         symmetry in Heqeq2.
-         inversion H2; subst.
-         intuition.
-         specialize (IHh1 _ _ _ _ _ Heqeq1 Heqeq2 H5).
-         subst. auto.
-       * inversion H1.
-       * inversion H0.
-       * inversion H0.
-Qed.
 
 
 (* = = = = = = = = = = = = = = = = = = = = = = = = = = = = = = = = *)
@@ -644,27 +539,38 @@ Proof.
     intuition.
 Qed.
 
+Lemma ast_ids_lt_add: forall ast_id n cks flag,
+    ast_id < n ->
+    ast_ids_lt cks n ->
+    ast_ids_lt ((ast_id, flag) :: cks) n.
+Proof.
+    intros.
+    constructor; auto.
+Qed.
+
 
 (** *** generate run-time-check flags for expressions *)
 (** compute check flags for each expression ast node according to the checking rules, and the results  
      are stored in a list of type check_points
 *)
 Inductive check_generator_expr: check_points -> expr -> check_points -> Prop :=
-    | CG_Econst: forall ast_id n flag ls,
-        check_flag (Econst ast_id n) flag -> 
-        check_generator_expr ls (Econst ast_id n) ((ast_id, flag ) :: ls)
-    | CG_Evar: forall ast_id x flag ls,
-        check_flag (Evar ast_id x) flag ->
-        check_generator_expr ls (Evar ast_id x) ((ast_id, flag) :: ls)
+    | CG_Econst: forall ast_id n ls,
+        check_generator_expr ls (Econst ast_id n) ls
+    | CG_Evar: forall ast_id x ls,
+        check_generator_expr ls (Evar ast_id x) ls
     | CG_Ebinop: forall ls e1 ls1 e2 ls2 ast_id op flag,
+        check_flag (Ebinop ast_id op e1 e2) (Some flag) -> 
+        check_generator_expr ((ast_id, flag) :: ls) e1 ls1 ->
+        check_generator_expr ls1 e2 ls2 ->
+        check_generator_expr ls (Ebinop ast_id op e1 e2) ls2
+    | CG_Ebinop_None: forall ls e1 ls1 e2 ls2 ast_id op,
+        check_flag (Ebinop ast_id op e1 e2) None -> 
         check_generator_expr ls e1 ls1 ->
         check_generator_expr ls1 e2 ls2 ->
-        check_flag (Ebinop ast_id op e1 e2) flag -> 
-        check_generator_expr ls (Ebinop ast_id op e1 e2) ((ast_id, flag) :: ls2)
-    | CG_Eunop: forall ls e ls1 ast_id op flag,
+        check_generator_expr ls (Ebinop ast_id op e1 e2) ls2
+    | CG_Eunop: forall ls e ls1 ast_id op,
         check_generator_expr ls e ls1 ->
-        check_flag (Eunop ast_id op e) flag ->
-        check_generator_expr ls (Eunop ast_id op e) ((ast_id, flag ) :: ls1).
+        check_generator_expr ls (Eunop ast_id op e) ls1.
 
 (** *** generate run-time-check flags for statements *)
 (** For the SPARK 2014 subset that we are working on, we only consider the division by zero check and 
@@ -674,28 +580,33 @@ Inductive check_generator_expr: check_points -> expr -> check_points -> Prop :=
 Inductive check_generator_stmt: check_points -> stmt -> check_points -> Prop :=
     | CG_Sassign: forall ls1 e ls2 ast_id x,
         check_generator_expr ls1 e ls2 ->
-        check_generator_stmt ls1 (Sassign ast_id x e) ((ast_id, No_Check) :: ls2)
+        check_generator_stmt ls1 (Sassign ast_id x e) ls2
     | CG_Sseq: forall ls1 c1 ls2 c2 ls3 ast_id,
         check_generator_stmt ls1 c1 ls2 ->
         check_generator_stmt ls2 c2 ls3 ->
-        check_generator_stmt ls1 (Sseq ast_id c1 c2) ((ast_id, No_Check) :: ls3)
+        check_generator_stmt ls1 (Sseq ast_id c1 c2) ls3
     | CG_Sifthen: forall ls1 b ls2 c ls3 ast_id,
         check_generator_expr ls1 b ls2 ->
         check_generator_stmt ls2 c ls3 ->
-        check_generator_stmt ls1 (Sifthen ast_id b c) ((ast_id, No_Check) :: ls3)
+        check_generator_stmt ls1 (Sifthen ast_id b c) ls3
     | CG_Swhile: forall ls1 b ls2 c ls3 ast_id,
         check_generator_expr ls1 b ls2 ->
         check_generator_stmt ls2 c ls3 ->        
-        check_generator_stmt ls1 (Swhile ast_id b c) ((ast_id, No_Check) :: ls3).
+        check_generator_stmt ls1 (Swhile ast_id b c) ls3.
 
 (** ** Semantics with run-time-checks *)
+(*
+Inductive correct_flag_on_op: check_action -> binary_operation -> Prop :=
+    | Div_Flag: correct_flag_on_op Do_Division_Check Odiv. 
+*)
+
 (** the semantics for expressions evaluation, where cps is passed in as a parameter telling 
      whether a check is needed to be performed before executing the expression ast node
 *)
 Inductive eval_expr_with_checks (cps: check_points): stack -> expr -> return_val -> Prop :=
     | eval_Const: forall cst v s ast_id,
         eval_constant cst = v ->
-        eval_expr_with_checks cps s (Econst ast_id cst) v
+        eval_expr_with_checks cps s (Econst ast_id cst) (ValNormal v)
     | eval_Var: forall x s v ast_id,
         fetch x s = Some v ->
         eval_expr_with_checks cps s (Evar ast_id x) (ValNormal v)
@@ -709,25 +620,29 @@ Inductive eval_expr_with_checks (cps: check_points): stack -> expr -> return_val
     | eval_Binop3: forall s e1 v1 e2 v2 ck ast_id op,
         eval_expr_with_checks cps s e1 (ValNormal v1) ->
         eval_expr_with_checks cps s e2 (ValNormal v2) ->
-        fetch_ck ast_id cps = Some ck -> 
-        do_check (eval_expr_with_checks cps) s ck false ->
+        fetch_ck ast_id cps = Some ck ->
+        do_check op v1 v2 false ->
         eval_expr_with_checks cps s (Ebinop ast_id op e1 e2) ValException
     | eval_Binop4: forall s e1 v1 e2 v2 ck ast_id op v,
         eval_expr_with_checks cps s e1 (ValNormal v1) ->
         eval_expr_with_checks cps s e2 (ValNormal v2) ->
         fetch_ck ast_id cps = Some ck -> 
-        do_check (eval_expr_with_checks cps) s ck true ->
-        eval_binop op (ValNormal v1) (ValNormal v2) = v ->
-        v <> ValAbnormal ->
-        eval_expr_with_checks cps s (Ebinop ast_id op e1 e2) v
+        do_check op v1 v2 true ->
+        eval_binexpr op v1 v2 v ->
+        eval_expr_with_checks cps s (Ebinop ast_id op e1 e2) (ValNormal v)
+    | eval_Binop5: forall s e1 v1 e2 v2 ast_id op v,
+        eval_expr_with_checks cps s e1 (ValNormal v1) ->
+        eval_expr_with_checks cps s e2 (ValNormal v2) ->
+        fetch_ck ast_id cps = None ->
+        eval_binexpr op v1 v2 v ->
+        eval_expr_with_checks cps s (Ebinop ast_id op e1 e2) (ValNormal v)
     | eval_Unop1: forall s e ast_id op,
         eval_expr_with_checks cps s e ValException ->
         eval_expr_with_checks cps s (Eunop ast_id op e) ValException
     | eval_Unop2: forall s e v ast_id op v1,
         eval_expr_with_checks cps s e (ValNormal v) ->
-        eval_unop op (ValNormal v) = v1 ->
-        v1 <> ValAbnormal ->
-        eval_expr_with_checks cps s (Eunop ast_id op e) v1.
+        eval_unaryexpr op v v1 ->
+        eval_expr_with_checks cps s (Eunop ast_id op e) (ValNormal v1).
 
 
 (** 
@@ -786,90 +701,10 @@ Proof.
     intros.
     induction H;
     try match goal with
-    | [ |- (exists v0 : value, ValNormal v = ValNormal v0) \/ _ ] => left; exists v; reflexivity
+    | [ |- (exists v0 : value, ValNormal ?v = ValNormal v0) \/ _ ] => left; exists v; reflexivity
     | [ |- _ \/ ?A = ?A ] => right; reflexivity
     end.
-  - destruct cst; simpl in H; rewrite <- H;
-    left; 
-    [exists (Int z) | exists (Bool b)]; reflexivity.
-  - destruct v.
-    left; exists v; reflexivity.
-    right; reflexivity.
-    intuition.
-  - destruct v1.
-    left; exists v0; reflexivity.
-    right; reflexivity.
-    intuition.    
 Qed.
-
-(** the results of running eval_expr_with_checks should be unique *)
-Lemma eval_expr_with_checks_unique: forall ls s e v1 v2,
-    eval_expr_with_checks ls s e (ValNormal v1) ->
-    eval_expr_with_checks ls s e (ValNormal v2) ->
-    v1 = v2.
-Proof.
-    induction e;
-    intros v1 v2 h1 h2;
-    inversion h1; subst;
-    inversion h2; subst.
-  - rewrite H3 in H4.
-    inversion H4; subst;
-    reflexivity.
-  - rewrite H1 in H2; inversion H2; subst; 
-    reflexivity.
-  - specialize (IHe1 _ _ H3 H5).
-    specialize (IHe2 _ _ H4 H7). subst.
-    rewrite H15 in H9; inversion H9; subst.
-    reflexivity.
-  - specialize (IHe _ _ H1 H2).
-    subst. 
-    destruct op0, op.
-    rewrite H6 in H3; inversion H3; subst;
-    auto.
-Qed.
-
-(*
-Lemma eval_expr_with_checks_unique: forall ls s e v1 v2,
-    eval_expr_with_checks ls s e v1 ->
-    eval_expr_with_checks ls s e v2 ->
-    v1 = v2.
-Proof.
-    induction e;
-    intros v1 v2 h1 h2.
-  - inversion h1; subst. 
-    inversion h2; subst.
-    reflexivity.
-  - inversion h1; subst. 
-    inversion h2; subst.
-    rewrite H3 in H4; inversion H4; subst; reflexivity.
-  - inversion h1; subst.
-    inversion h2; subst; auto;
-    repeat match goal with
-    | [ h1:  forall v1 v2,
-               eval_expr_with_checks ?ls ?s ?e v1 ->
-               eval_expr_with_checks ?ls ?s ?e v2 -> v1 = v2, 
-        h2: eval_expr_with_checks ?ls ?s ?e ?x,
-        h3: eval_expr_with_checks ?ls ?s ?e ?y |- _ ] => specialize (h1 _ _ h2 h3); inversion h1; subst
-    end; auto.
-    rewrite H7 in H10. inversion H10; subst. 
-    clear IHe2 IHe1 H6 H4 H10.
-    
-    inversion H8; subst.
-    inversion H8; subst.
-    inversion H12; subst.   
-    
-    - inversion h1; subst;
-      inversion h2; subst; auto;
-      match goal with
-      | [ h1:  forall v1 v2,
-               eval_expr_with_checks ?ls ?s ?e v1 ->
-               eval_expr_with_checks ?ls ?s ?e v2 -> v1 = v2, 
-        h2: eval_expr_with_checks ?ls ?s ?e ?x,
-        h3: eval_expr_with_checks ?ls ?s ?e ?y |- _ ] => specialize (h1 _ _ h2 h3); inversion h1; subst
-    end; auto.
-    destruct op, op0; auto.
-Qed.
-*)
 
 (** 
    the ast id number is increasing: parent node's ast id number is smaller than children node's ast id number.
@@ -901,28 +736,24 @@ Proof.
     induction h1;
     intros cks0 cks h2 h3;
     simpl in h3; inversion h2; subst.
-  - constructor.
-    apply ast_ids_lt_trans with (n := ast_id); intuition.
-    intuition.
-  - constructor.
-    apply ast_ids_lt_trans with (n := ast_id); intuition.
-    intuition.
+  - apply ast_ids_lt_trans with (n := ast_id); intuition.
+  - apply ast_ids_lt_trans with (n := ast_id); intuition.
   - specialize (ast_ids_lt_trans _ _ _ h3 H1); intros hz1.
-    specialize (ast_ids_lt_trans _ _ _ h3 H2); intros hz2.
-    specialize (IHh1_1 _ _ H10 hz1).
+    specialize (ast_ids_lt_add _ _ _ flag H1 hz1); intros hz2.
+    specialize (IHh1_1 _ _ H11 hz2).
     assert(hz: max1 + 1 <= get_ast_id_expr e2); intuition.
     specialize (ast_ids_lt_trans0 _ _ _ IHh1_1 hz); intros hz3.
-    specialize (IHh1_2 _ _ H11 hz3).
-    constructor.
-    + assumption.
-    + specialize (ast_id_bound_expr _ _ h1_2); intros hz4.
-       intuition.
+    specialize (IHh1_2 _ _ H12 hz3).
+    assumption.
+  - specialize (ast_ids_lt_trans _ _ _ h3 H1); intros hz1.
+    specialize (IHh1_1 _ _ H11 hz1).
+    assert(hz: max1 + 1 <= get_ast_id_expr e2); intuition.
+    specialize (ast_ids_lt_trans0 _ _ _ IHh1_1 hz); intros hz3.
+    specialize (IHh1_2 _ _ H12 hz3).
+    assumption.
   - specialize (ast_ids_lt_trans _ _ _ h3 H0); intros hz1.
-    specialize (IHh1 _ _ H4 hz1).
-    constructor.
-    + assumption.
-    + specialize (ast_id_bound_expr _ _ h1); intros hz2.
-       intuition.
+    specialize (IHh1 _ _ H5 hz1).
+    assumption.
 Qed.
 
 (** it's similar to ast_id_bound_expr *)
@@ -950,32 +781,25 @@ Proof.
     simpl in h3; inversion h2; subst.
   - specialize (ast_ids_lt_trans _ _ _ h3 H1); intros hz1.
     specialize (ast_id_max_expr _ _ _ _ H H7 hz1); intros hz2.
-    specialize (ast_id_bound_expr _ _ H); intros hz3.
-    constructor; intuition.
+    assumption.
   - specialize (ast_ids_lt_trans _ _ _ h3 H1); intros hz1.
     specialize (IHh1_1 _ _ H9 hz1).
     assert (hz: max1 + 1 <= get_ast_id_stmt c2); intuition.
     specialize (ast_ids_lt_trans0 _ _ _ IHh1_1 hz); intros hz2.
     specialize (IHh1_2 _ _ H10 hz2).
-    constructor. assumption.
-    specialize (ast_id_bound_stmt _ _ h1_2); intros hz3.
-    intuition.
+    assumption.
   - specialize (ast_ids_lt_trans _ _ _ h3 H2); intros hz1.
     specialize (ast_id_max_expr _ _ _ _ H H10 hz1); intros hz2.
     assert (hz: max1 + 1 <= get_ast_id_stmt c); intuition.
     specialize (ast_ids_lt_trans0 _ _ _ hz2 hz); intros hz3.
     specialize (IHh1 _ _ H11 hz3).
-    constructor. assumption.
-    specialize (ast_id_bound_stmt _ _ h1); intros hz4.
-    intuition.
+    assumption.
   - specialize (ast_ids_lt_trans _ _ _ h3 H2); intros hz1.
     specialize (ast_id_max_expr _ _ _ _ H H10 hz1); intros hz2.
     assert (hz: max1 + 1 <= get_ast_id_stmt c); intuition.
     specialize (ast_ids_lt_trans0 _ _ _ hz2 hz); intros hz3.
     specialize (IHh1 _ _ H11 hz3).
-    constructor. assumption.
-    specialize (ast_id_bound_stmt _ _ h1); intros hz4.
-    intuition.
+    assumption.
 Qed.
 
 
